pass on proof/amd64

proof/amd64/extracted/Keccak1600_Jazz_ASIZE.ec
@@ -5,8 +5,8 @@ from Jasmin require import JModel_x86.
 import SLH64.
 
 require import
-Array5 Array6 Array7 Array24 Array25 Array999 WArray160 WArray192 WArray200
-WArray224 WArray800 WArray999.
+Array5 Array6 Array7 Array24 Array25 Array999 WArray40 WArray160 WArray192
+WArray200 WArray224 WArray800 WArray999.
 
 abbrev rOL8 =
 (W256.of_int
@@ -51,6 +51,393 @@ abbrev kECCAK1600_RC =
 (W64.of_int (-9223372034707259384))]).
 
 module M = {
+  proc __SHLQ (x:W64.t, shbytes:int) : W64.t = {
+    
+    if ((shbytes <> 0)) {
+      x <- (x `<<` (W8.of_int (8 * shbytes)));
+    } else {
+      
+    }
+    return x;
+  }
+  proc __SHLDQ (x:W128.t, shbytes:int) : W128.t = {
+    
+    if ((shbytes <> 0)) {
+      x <- (VPSLLDQ_128 x (W8.of_int shbytes));
+    } else {
+      
+    }
+    return x;
+  }
+  proc __SHLQ_256 (x:W256.t, shbytes:int) : W256.t = {
+    
+    if ((shbytes <> 0)) {
+      x <- (VPSLL_4u64 x (W128.of_int (8 * shbytes)));
+    } else {
+      
+    }
+    return x;
+  }
+  proc __m_ilen_read_upto8_at (buf:int, lEN:int, tRAIL:int, cUR:int, aT:int) : 
+  int * int * int * int * W64.t = {
+    var w:W64.t;
+    var aT8:int;
+    var t16:W64.t;
+    var t8:W64.t;
+    if ((((aT < cUR) \/ ((cUR + 8) <= aT)) \/ ((lEN = 0) /\ (tRAIL = 0)))) {
+      w <- (W64.of_int 0);
+    } else {
+      aT8 <- (aT - cUR);
+      if ((8 <= lEN)) {
+        w <- (loadW64 Glob.mem buf);
+        w <@ __SHLQ (w, aT8);
+        buf <- (buf + (8 - aT8));
+        lEN <- (lEN - (8 - aT8));
+        aT8 <- 8;
+      } else {
+        if ((4 <= lEN)) {
+          w <- (zeroextu64 (loadW32 Glob.mem buf));
+          w <@ __SHLQ (w, aT8);
+          buf <- (buf + ((8 <= (4 + aT8)) ? (8 - aT8) : 4));
+          lEN <- (lEN - ((8 <= (4 + aT8)) ? (8 - aT8) : 4));
+          aT8 <- ((8 <= (4 + aT8)) ? 8 : (4 + aT8));
+        } else {
+          w <- (W64.of_int 0);
+        }
+        if (((aT8 < 8) /\ (2 <= lEN))) {
+          t16 <- (zeroextu64 (loadW16 Glob.mem buf));
+          buf <- (buf + ((8 <= (2 + aT8)) ? (8 - aT8) : 2));
+          lEN <- (lEN - ((8 <= (2 + aT8)) ? (8 - aT8) : 2));
+          t16 <@ __SHLQ (t16, aT8);
+          w <- (w `|` t16);
+          aT8 <- ((8 <= (2 + aT8)) ? 8 : (2 + aT8));
+        } else {
+          
+        }
+        if ((aT8 < 8)) {
+          if ((1 <= lEN)) {
+            t8 <- (zeroextu64 (loadW8 Glob.mem buf));
+            t8 <- (t8 `|` (W64.of_int (256 * (tRAIL %% 256))));
+            buf <- (buf + 1);
+            lEN <- (lEN - 1);
+            t8 <@ __SHLQ (t8, aT8);
+            w <- (w `|` t8);
+            aT8 <- (aT8 + 1);
+            if (((aT8 < 8) /\ ((tRAIL %% 256) <> 0))) {
+              aT8 <- (aT8 + 1);
+              tRAIL <- 0;
+            } else {
+              
+            }
+          } else {
+            if (((tRAIL %% 256) <> 0)) {
+              t8 <- (W64.of_int (tRAIL %% 256));
+              t8 <@ __SHLQ (t8, aT8);
+              w <- (w `|` t8);
+              tRAIL <- 0;
+              aT8 <- (aT8 + 1);
+            } else {
+              
+            }
+          }
+        } else {
+          
+        }
+      }
+      aT <- (cUR + aT8);
+    }
+    return (buf, lEN, tRAIL, aT, w);
+  }
+  proc __m_ilen_read_upto16_at (buf:int, lEN:int, tRAIL:int, cUR:int, aT:int) : 
+  int * int * int * int * W128.t = {
+    var w:W128.t;
+    var aT16:int;
+    var t64_0:W64.t;
+    var t64_1:W64.t;
+    if ((((aT < cUR) \/ ((cUR + 16) <= aT)) \/ ((lEN = 0) /\ (tRAIL = 0)))) {
+      w <- (set0_128);
+    } else {
+      aT16 <- (aT - cUR);
+      if ((16 <= lEN)) {
+        w <- (loadW128 Glob.mem buf);
+        w <@ __SHLDQ (w, aT16);
+        buf <- (buf + (16 - aT16));
+        lEN <- (lEN - (16 - aT16));
+        aT16 <- 16;
+      } else {
+        if ((8 <= aT16)) {
+          w <- (set0_128);
+          (buf, lEN, tRAIL, aT16, t64_1) <@ __m_ilen_read_upto8_at (buf, 
+          lEN, tRAIL, 8, aT16);
+          w <- (VPINSR_2u64 w t64_1 (W8.of_int 1));
+        } else {
+          (buf, lEN, tRAIL, aT16, t64_0) <@ __m_ilen_read_upto8_at (buf, 
+          lEN, tRAIL, 0, aT16);
+          w <- (zeroextu128 t64_0);
+          (buf, lEN, tRAIL, aT16, t64_1) <@ __m_ilen_read_upto8_at (buf, 
+          lEN, tRAIL, 8, aT16);
+          w <- (VPINSR_2u64 w t64_1 (W8.of_int 1));
+        }
+      }
+      aT <- (cUR + aT16);
+    }
+    return (buf, lEN, tRAIL, aT, w);
+  }
+  proc __m_ilen_read_upto32_at (buf:int, lEN:int, tRAIL:int, cUR:int, aT:int) : 
+  int * int * int * int * W256.t = {
+    var w:W256.t;
+    var aT32:int;
+    var t128_0:W128.t;
+    var t128_1:W128.t;
+    if ((((aT < cUR) \/ ((cUR + 32) <= aT)) \/ ((lEN = 0) /\ (tRAIL = 0)))) {
+      w <- (set0_256);
+    } else {
+      aT32 <- (aT - cUR);
+      if (((aT32 = 0) /\ (32 <= lEN))) {
+        w <- (loadW256 Glob.mem buf);
+        aT32 <- (aT32 + 32);
+        buf <- (buf + 32);
+        lEN <- (lEN - 32);
+      } else {
+        if ((16 <= aT32)) {
+          w <- (set0_256);
+          (buf, lEN, tRAIL, aT32, t128_1) <@ __m_ilen_read_upto16_at (
+          buf, lEN, tRAIL, 16, aT32);
+          w <- (VINSERTI128 w t128_1 (W8.of_int 1));
+        } else {
+          (buf, lEN, tRAIL, aT32, t128_0) <@ __m_ilen_read_upto16_at (
+          buf, lEN, tRAIL, 0, aT32);
+          (buf, lEN, tRAIL, aT32, t128_1) <@ __m_ilen_read_upto16_at (
+          buf, lEN, tRAIL, 16, aT32);
+          w <-
+          (W256.of_int
+          (((W128.to_uint t128_0) %% (2 ^ 128)) +
+          ((2 ^ 128) * (W128.to_uint t128_1))));
+        }
+      }
+      aT <- (cUR + aT32);
+    }
+    return (buf, lEN, tRAIL, aT, w);
+  }
+  proc __m_ilen_read_bcast_upto8_at (buf:int, lEN:int, tRAIL:int, cUR:int,
+                                     aT:int) : int * int * int * int * W256.t = {
+    var w256:W256.t;
+    var aT8:int;
+    var w:W64.t;
+    var t128:W128.t;
+    if ((((aT < cUR) \/ ((cUR + 8) <= aT)) \/ ((lEN = 0) /\ (tRAIL = 0)))) {
+      w256 <- (set0_256);
+    } else {
+      if ((8 <= lEN)) {
+        aT8 <- (aT - cUR);
+        w256 <- (VPBROADCAST_4u64 (loadW64 Glob.mem buf));
+        w256 <@ __SHLQ_256 (w256, aT8);
+        buf <- (buf + (8 - aT8));
+        lEN <- (lEN - (8 - aT8));
+        aT8 <- 8;
+      } else {
+        aT8 <- (aT - cUR);
+        (buf, lEN, tRAIL, aT, w) <@ __m_ilen_read_upto8_at (buf, lEN, 
+        tRAIL, cUR, aT);
+        t128 <- (zeroextu128 w);
+        w256 <- (VPBROADCAST_4u64 (truncateu64 t128));
+        w256 <@ __SHLQ_256 (w256, aT8);
+        buf <- (buf + (8 - aT8));
+        lEN <- (lEN - (8 - aT8));
+        aT8 <- 8;
+      }
+      aT <- (cUR + aT8);
+    }
+    return (buf, lEN, tRAIL, aT, w256);
+  }
+  proc __m_ilen_write_upto8 (buf:int, lEN:int, w:W64.t) : int * int = {
+    
+    if ((0 < lEN)) {
+      if ((8 <= lEN)) {
+        Glob.mem <- (storeW64 Glob.mem buf w);
+        buf <- (buf + 8);
+        lEN <- (lEN - 8);
+      } else {
+        if ((4 <= lEN)) {
+          Glob.mem <- (storeW32 Glob.mem buf (truncateu32 w));
+          w <- (w `>>` (W8.of_int 32));
+          buf <- (buf + 4);
+          lEN <- (lEN - 4);
+        } else {
+          
+        }
+        if ((2 <= lEN)) {
+          Glob.mem <- (storeW16 Glob.mem buf (truncateu16 w));
+          w <- (w `>>` (W8.of_int 16));
+          buf <- (buf + 2);
+          lEN <- (lEN - 2);
+        } else {
+          
+        }
+        if ((1 <= lEN)) {
+          Glob.mem <- (storeW8 Glob.mem buf (truncateu8 w));
+          buf <- (buf + 1);
+          lEN <- (lEN - 1);
+        } else {
+          
+        }
+      }
+    } else {
+      
+    }
+    return (buf, lEN);
+  }
+  proc __m_ilen_write_upto16 (buf:int, lEN:int, w:W128.t) : int * int = {
+    var t64:W64.t;
+    if ((0 < lEN)) {
+      if ((16 <= lEN)) {
+        Glob.mem <- (storeW128 Glob.mem buf w);
+        buf <- (buf + 16);
+        lEN <- (lEN - 16);
+      } else {
+        if ((8 <= lEN)) {
+          Glob.mem <- (storeW64 Glob.mem buf (MOVV_64 (truncateu64 w)));
+          buf <- (buf + 8);
+          lEN <- (lEN - 8);
+          w <- (VPUNPCKH_2u64 w w);
+        } else {
+          
+        }
+        t64 <- (truncateu64 w);
+        (buf, lEN) <@ __m_ilen_write_upto8 (buf, lEN, t64);
+      }
+    } else {
+      
+    }
+    return (buf, lEN);
+  }
+  proc __m_ilen_write_upto32 (buf:int, lEN:int, w:W256.t) : int * int = {
+    var t128:W128.t;
+    if ((0 < lEN)) {
+      if ((32 <= lEN)) {
+        Glob.mem <- (storeW256 Glob.mem buf w);
+        buf <- (buf + 32);
+        lEN <- (lEN - 32);
+      } else {
+        t128 <- (truncateu128 w);
+        if ((16 <= lEN)) {
+          Glob.mem <- (storeW128 Glob.mem buf t128);
+          buf <- (buf + 16);
+          lEN <- (lEN - 16);
+          t128 <- (VEXTRACTI128 w (W8.of_int 1));
+        } else {
+          
+        }
+        (buf, lEN) <@ __m_ilen_write_upto16 (buf, lEN, t128);
+      }
+    } else {
+      
+    }
+    return (buf, lEN);
+  }
+  proc __m_rlen_read_upto8 (buf:int, len:int) : int * W64.t = {
+    var w:W64.t;
+    var zf:bool;
+    var sh:W8.t;
+    var x:W64.t;
+    var  _0:bool;
+    var  _1:bool;
+    var  _2:bool;
+    var  _3:bool;
+    var  _4:bool;
+    var  _5:bool;
+    var  _6:bool;
+    var  _7:bool;
+    var  _8:bool;
+    var  _9:bool;
+    var  _10:bool;
+    var  _11:bool;
+    if ((8 <= len)) {
+      w <- (loadW64 Glob.mem buf);
+      buf <- (buf + 8);
+    } else {
+      ( _0,  _1,  _2,  _3, zf) <- (TEST_64 (W64.of_int len) (W64.of_int 4));
+      if ((! zf)) {
+        w <- (zeroextu64 (loadW32 Glob.mem buf));
+        buf <- (buf + 4);
+        sh <- (W8.of_int 32);
+      } else {
+        w <- (W64.of_int 0);
+        sh <- (W8.of_int 0);
+      }
+      ( _4,  _5,  _6,  _7, zf) <- (TEST_64 (W64.of_int len) (W64.of_int 2));
+      if ((! zf)) {
+        x <- (zeroextu64 (loadW16 Glob.mem buf));
+        x <- (x `<<` (sh `&` (W8.of_int 63)));
+        w <- (w + x);
+        buf <- (buf + 2);
+        sh <- (sh + (W8.of_int 16));
+      } else {
+        
+      }
+      ( _8,  _9,  _10,  _11, zf) <-
+      (TEST_64 (W64.of_int len) (W64.of_int 1));
+      if ((! zf)) {
+        x <- (zeroextu64 (loadW8 Glob.mem buf));
+        x <- (x `<<` (sh `&` (W8.of_int 63)));
+        w <- (w + x);
+        buf <- (buf + 1);
+      } else {
+        
+      }
+    }
+    return (buf, w);
+  }
+  proc __m_rlen_write_upto8 (buf:int, data:W64.t, len:int) : int = {
+    var zf:bool;
+    var  _0:bool;
+    var  _1:bool;
+    var  _2:bool;
+    var  _3:bool;
+    var  _4:bool;
+    var  _5:bool;
+    var  _6:bool;
+    var  _7:bool;
+    var  _8:bool;
+    var  _9:bool;
+    var  _10:bool;
+    var  _11:bool;
+    if ((8 <= len)) {
+      Glob.mem <- (storeW64 Glob.mem buf data);
+      buf <- (buf + 8);
+    } else {
+      ( _0,  _1,  _2,  _3, zf) <- (TEST_64 (W64.of_int len) (W64.of_int 4));
+      if ((! zf)) {
+        Glob.mem <- (storeW32 Glob.mem buf (truncateu32 data));
+        buf <- (buf + 4);
+        data <- (data `>>` (W8.of_int 32));
+      } else {
+        
+      }
+      ( _4,  _5,  _6,  _7, zf) <- (TEST_64 (W64.of_int len) (W64.of_int 2));
+      if ((! zf)) {
+        Glob.mem <- (storeW16 Glob.mem buf (truncateu16 data));
+        buf <- (buf + 2);
+        data <- (data `>>` (W8.of_int 16));
+      } else {
+        
+      }
+      ( _8,  _9,  _10,  _11, zf) <-
+      (TEST_64 (W64.of_int len) (W64.of_int 1));
+      if ((! zf)) {
+        Glob.mem <- (storeW8 Glob.mem buf (truncateu8 data));
+        buf <- (buf + 1);
+      } else {
+        
+      }
+    }
+    return buf;
+  }
+  proc __ANDN_64 (a:W64.t, b:W64.t) : W64.t = {
+    var t:W64.t;
+    t <- ((invw a) `&` b);
+    return t;
+  }
   proc keccakf1600_index (x:int, y:int) : int = {
     var r:int;
     r <- ((x %% 5) + (5 * (y %% 5)));
@@ -85,6 +472,179 @@ module M = {
     i <@ keccakf1600_index (x, y);
     r <@ keccakf1600_rho_offsets (i);
     return r;
+  }
+  proc __rol_u64_ref (x:W64.t, i:int) : W64.t = {
+    var  _0:bool;
+    var  _1:bool;
+    if ((i <> 0)) {
+      ( _0,  _1, x) <- (ROL_64 x (W8.of_int i));
+    } else {
+      
+    }
+    return x;
+  }
+  proc __theta_sum_ref (a:W64.t Array25.t) : W64.t Array5.t = {
+    var c:W64.t Array5.t;
+    var x:int;
+    var y:int;
+    c <- witness;
+    x <- 0;
+    while ((x < 5)) {
+      c.[x] <- a.[(x + 0)];
+      x <- (x + 1);
+    }
+    y <- 1;
+    while ((y < 5)) {
+      x <- 0;
+      while ((x < 5)) {
+        c.[x] <- (c.[x] `^` a.[(x + (y * 5))]);
+        x <- (x + 1);
+      }
+      y <- (y + 1);
+    }
+    return c;
+  }
+  proc __theta_rol_ref (c:W64.t Array5.t) : W64.t Array5.t = {
+    var aux:W64.t;
+    var d:W64.t Array5.t;
+    var x:int;
+    d <- witness;
+    x <- 0;
+    while ((x < 5)) {
+      d.[x] <- c.[((x + 1) %% 5)];
+      aux <@ __rol_u64_ref (d.[x], 1);
+      d.[x] <- aux;
+      d.[x] <- (d.[x] `^` c.[(((x - 1) + 5) %% 5)]);
+      x <- (x + 1);
+    }
+    return d;
+  }
+  proc __rol_sum_ref (a:W64.t Array25.t, d:W64.t Array5.t, y:int) : W64.t Array5.t = {
+    var aux:W64.t;
+    var b:W64.t Array5.t;
+    var x:int;
+    var x_:int;
+    var y_:int;
+    var r:int;
+    b <- witness;
+    x <- 0;
+    while ((x < 5)) {
+      x_ <- ((x + (3 * y)) %% 5);
+      y_ <- x;
+      r <@ keccakf1600_rhotates (x_, y_);
+      b.[x] <- a.[(x_ + (y_ * 5))];
+      b.[x] <- (b.[x] `^` d.[x_]);
+      aux <@ __rol_u64_ref (b.[x], r);
+      b.[x] <- aux;
+      x <- (x + 1);
+    }
+    return b;
+  }
+  proc __set_row_ref (e:W64.t Array25.t, b:W64.t Array5.t, y:int) : W64.t Array25.t = {
+    var x:int;
+    var x1:int;
+    var x2:int;
+    var t:W64.t;
+    x <- 0;
+    while ((x < 5)) {
+      x1 <- ((x + 1) %% 5);
+      x2 <- ((x + 2) %% 5);
+      t <@ __ANDN_64 (b.[x1], b.[x2]);
+      t <- (t `^` b.[x]);
+      e.[(x + (y * 5))] <- t;
+      x <- (x + 1);
+    }
+    return e;
+  }
+  proc _pround_ref (e:W64.t Array25.t, a:W64.t Array25.t) : W64.t Array25.t = {
+    var c:W64.t Array5.t;
+    var d:W64.t Array5.t;
+    var y:int;
+    var b:W64.t Array5.t;
+    b <- witness;
+    c <- witness;
+    d <- witness;
+    c <@ __theta_sum_ref (a);
+    d <@ __theta_rol_ref (c);
+    y <- 0;
+    while ((y < 5)) {
+      b <@ __rol_sum_ref (a, d, y);
+      e <@ __set_row_ref (e, b, y);
+      y <- (y + 1);
+    }
+    return e;
+  }
+  proc __keccakf1600_ref (a:W64.t Array25.t) : W64.t Array25.t = {
+    var s_e:W64.t Array25.t;
+    var e:W64.t Array25.t;
+    var rC:W64.t Array24.t;
+    var rc:W64.t;
+    var c:int;
+    rC <- witness;
+    e <- witness;
+    s_e <- witness;
+    e <- s_e;
+    c <- 0;
+    (* Erased call to spill *)
+    e <@ _pround_ref (e, a);
+    (a, e) <- (swap_ e a);
+    rC <- kECCAK1600_RC;
+    rc <- rC.[c];
+    e.[0] <- (e.[0] `^` rc);
+    a <@ _pround_ref (a, e);
+    (a, e) <- (swap_ e a);
+    rC <- kECCAK1600_RC;
+    rc <- rC.[(c + 1)];
+    a.[0] <- (a.[0] `^` rc);
+    (* Erased call to unspill *)
+    c <- (c + 2);
+    while ((c < (24 - 1))) {
+      (* Erased call to spill *)
+      e <@ _pround_ref (e, a);
+      (a, e) <- (swap_ e a);
+      rC <- kECCAK1600_RC;
+      rc <- rC.[c];
+      e.[0] <- (e.[0] `^` rc);
+      a <@ _pround_ref (a, e);
+      (a, e) <- (swap_ e a);
+      rC <- kECCAK1600_RC;
+      rc <- rC.[(c + 1)];
+      a.[0] <- (a.[0] `^` rc);
+      (* Erased call to unspill *)
+      c <- (c + 2);
+    }
+    return a;
+  }
+  proc _keccakf1600_ref (a:W64.t Array25.t) : W64.t Array25.t = {
+    
+    a <@ __keccakf1600_ref (a);
+    return a;
+  }
+  proc _keccakf1600_ref_ (a:W64.t Array25.t) : W64.t Array25.t = {
+    
+    a <- a;
+    a <@ _keccakf1600_ref (a);
+    a <- a;
+    return a;
+  }
+  proc __state_init_ref (st:W64.t Array25.t) : W64.t Array25.t = {
+    var z64:W64.t;
+    var i:int;
+    z64 <- (W64.of_int 0);
+    i <- 0;
+    while ((i < 25)) {
+      st.[i] <- z64;
+      i <- (i + 1);
+    }
+    return st;
+  }
+  proc __addratebit_ref (st:W64.t Array25.t, _RATE8:int) : W64.t Array25.t = {
+    var t64:W64.t;
+    t64 <- (W64.of_int 1);
+    t64 <- (t64 `<<` (W8.of_int (((8 * _RATE8) - 1) %% 64)));
+    t64 <- (t64 `^` st.[((_RATE8 - 1) %/ 8)]);
+    st.[((_RATE8 - 1) %/ 8)] <- t64;
+    return st;
   }
   proc __keccakf1600_pround_avx2 (state:W256.t Array7.t) : W256.t Array7.t = {
     var c00:W256.t;
@@ -1107,388 +1667,6 @@ module M = {
     st25 <@ __stavx2_unpack (st25, state);
     return st25;
   }
-  proc __SHLQ (x:W64.t, shbytes:int) : W64.t = {
-    
-    if ((shbytes <> 0)) {
-      x <- (x `<<` (W8.of_int (8 * shbytes)));
-    } else {
-      
-    }
-    return x;
-  }
-  proc __SHLDQ (x:W128.t, shbytes:int) : W128.t = {
-    
-    if ((shbytes <> 0)) {
-      x <- (VPSLLDQ_128 x (W8.of_int shbytes));
-    } else {
-      
-    }
-    return x;
-  }
-  proc __SHLQ_256 (x:W256.t, shbytes:int) : W256.t = {
-    
-    if ((shbytes <> 0)) {
-      x <- (VPSLL_4u64 x (W128.of_int (8 * shbytes)));
-    } else {
-      
-    }
-    return x;
-  }
-  proc __m_ilen_read_upto8_at (buf:int, lEN:int, tRAIL:int, cUR:int, aT:int) : 
-  int * int * int * int * W64.t = {
-    var w:W64.t;
-    var aT8:int;
-    var t16:W64.t;
-    var t8:W64.t;
-    if ((((aT < cUR) \/ ((cUR + 8) <= aT)) \/ ((lEN = 0) /\ (tRAIL = 0)))) {
-      w <- (W64.of_int 0);
-    } else {
-      aT8 <- (aT - cUR);
-      if ((8 <= lEN)) {
-        w <- (loadW64 Glob.mem buf);
-        w <@ __SHLQ (w, aT8);
-        buf <- (buf + (8 - aT8));
-        lEN <- (lEN - (8 - aT8));
-        aT8 <- 8;
-      } else {
-        if ((4 <= lEN)) {
-          w <- (zeroextu64 (loadW32 Glob.mem buf));
-          w <@ __SHLQ (w, aT8);
-          buf <- (buf + ((8 <= (4 + aT8)) ? (8 - aT8) : 4));
-          lEN <- (lEN - ((8 <= (4 + aT8)) ? (8 - aT8) : 4));
-          aT8 <- ((8 <= (4 + aT8)) ? 8 : (4 + aT8));
-        } else {
-          w <- (W64.of_int 0);
-        }
-        if (((aT8 < 8) /\ (2 <= lEN))) {
-          t16 <- (zeroextu64 (loadW16 Glob.mem buf));
-          buf <- (buf + ((8 <= (2 + aT8)) ? (8 - aT8) : 2));
-          lEN <- (lEN - ((8 <= (2 + aT8)) ? (8 - aT8) : 2));
-          t16 <@ __SHLQ (t16, aT8);
-          w <- (w `|` t16);
-          aT8 <- ((8 <= (2 + aT8)) ? 8 : (2 + aT8));
-        } else {
-          
-        }
-        if ((aT8 < 8)) {
-          if ((1 <= lEN)) {
-            t8 <- (zeroextu64 (loadW8 Glob.mem buf));
-            t8 <- (t8 `|` (W64.of_int (256 * (tRAIL %% 256))));
-            buf <- (buf + 1);
-            lEN <- (lEN - 1);
-            t8 <@ __SHLQ (t8, aT8);
-            w <- (w `|` t8);
-            aT8 <- (aT8 + 1);
-            if (((aT8 < 8) /\ ((tRAIL %% 256) <> 0))) {
-              aT8 <- (aT8 + 1);
-              tRAIL <- 0;
-            } else {
-              
-            }
-          } else {
-            if (((tRAIL %% 256) <> 0)) {
-              t8 <- (W64.of_int (tRAIL %% 256));
-              t8 <@ __SHLQ (t8, aT8);
-              w <- (w `|` t8);
-              tRAIL <- 0;
-              aT8 <- (aT8 + 1);
-            } else {
-              
-            }
-          }
-        } else {
-          
-        }
-      }
-      aT <- (cUR + aT8);
-    }
-    return (buf, lEN, tRAIL, aT, w);
-  }
-  proc __m_ilen_read_upto16_at (buf:int, lEN:int, tRAIL:int, cUR:int, aT:int) : 
-  int * int * int * int * W128.t = {
-    var w:W128.t;
-    var aT16:int;
-    var t64_0:W64.t;
-    var t64_1:W64.t;
-    if ((((aT < cUR) \/ ((cUR + 16) <= aT)) \/ ((lEN = 0) /\ (tRAIL = 0)))) {
-      w <- (set0_128);
-    } else {
-      aT16 <- (aT - cUR);
-      if ((16 <= lEN)) {
-        w <- (loadW128 Glob.mem buf);
-        w <@ __SHLDQ (w, aT16);
-        buf <- (buf + (16 - aT16));
-        lEN <- (lEN - (16 - aT16));
-        aT16 <- 16;
-      } else {
-        if ((8 <= aT16)) {
-          w <- (set0_128);
-          (buf, lEN, tRAIL, aT16, t64_1) <@ __m_ilen_read_upto8_at (buf, 
-          lEN, tRAIL, 8, aT16);
-          w <- (VPINSR_2u64 w t64_1 (W8.of_int 1));
-        } else {
-          (buf, lEN, tRAIL, aT16, t64_0) <@ __m_ilen_read_upto8_at (buf, 
-          lEN, tRAIL, 0, aT16);
-          w <- (zeroextu128 t64_0);
-          (buf, lEN, tRAIL, aT16, t64_1) <@ __m_ilen_read_upto8_at (buf, 
-          lEN, tRAIL, 8, aT16);
-          w <- (VPINSR_2u64 w t64_1 (W8.of_int 1));
-        }
-      }
-      aT <- (cUR + aT16);
-    }
-    return (buf, lEN, tRAIL, aT, w);
-  }
-  proc __m_ilen_read_upto32_at (buf:int, lEN:int, tRAIL:int, cUR:int, aT:int) : 
-  int * int * int * int * W256.t = {
-    var w:W256.t;
-    var aT32:int;
-    var t128_0:W128.t;
-    var t128_1:W128.t;
-    if ((((aT < cUR) \/ ((cUR + 32) <= aT)) \/ ((lEN = 0) /\ (tRAIL = 0)))) {
-      w <- (set0_256);
-    } else {
-      aT32 <- (aT - cUR);
-      if (((aT32 = 0) /\ (32 <= lEN))) {
-        w <- (loadW256 Glob.mem buf);
-        aT32 <- (aT32 + 32);
-        buf <- (buf + 32);
-        lEN <- (lEN - 32);
-      } else {
-        if ((16 <= aT32)) {
-          w <- (set0_256);
-          (buf, lEN, tRAIL, aT32, t128_1) <@ __m_ilen_read_upto16_at (
-          buf, lEN, tRAIL, 16, aT32);
-          w <- (VINSERTI128 w t128_1 (W8.of_int 1));
-        } else {
-          (buf, lEN, tRAIL, aT32, t128_0) <@ __m_ilen_read_upto16_at (
-          buf, lEN, tRAIL, 0, aT32);
-          (buf, lEN, tRAIL, aT32, t128_1) <@ __m_ilen_read_upto16_at (
-          buf, lEN, tRAIL, 16, aT32);
-          w <-
-          (W256.of_int
-          (((W128.to_uint t128_0) %% (2 ^ 128)) +
-          ((2 ^ 128) * (W128.to_uint t128_1))));
-        }
-      }
-      aT <- (cUR + aT32);
-    }
-    return (buf, lEN, tRAIL, aT, w);
-  }
-  proc __m_ilen_read_bcast_upto8_at (buf:int, lEN:int, tRAIL:int, cUR:int,
-                                     aT:int) : int * int * int * int * W256.t = {
-    var w256:W256.t;
-    var aT8:int;
-    var w:W64.t;
-    var t128:W128.t;
-    if ((((aT < cUR) \/ ((cUR + 8) <= aT)) \/ ((lEN = 0) /\ (tRAIL = 0)))) {
-      w256 <- (set0_256);
-    } else {
-      if ((8 <= lEN)) {
-        aT8 <- (aT - cUR);
-        w256 <- (VPBROADCAST_4u64 (loadW64 Glob.mem buf));
-        w256 <@ __SHLQ_256 (w256, aT8);
-        buf <- (buf + (8 - aT8));
-        lEN <- (lEN - (8 - aT8));
-        aT8 <- 8;
-      } else {
-        aT8 <- (aT - cUR);
-        (buf, lEN, tRAIL, aT, w) <@ __m_ilen_read_upto8_at (buf, lEN, 
-        tRAIL, cUR, aT);
-        t128 <- (zeroextu128 w);
-        w256 <- (VPBROADCAST_4u64 (truncateu64 t128));
-        w256 <@ __SHLQ_256 (w256, aT8);
-        buf <- (buf + (8 - aT8));
-        lEN <- (lEN - (8 - aT8));
-        aT8 <- 8;
-      }
-      aT <- (cUR + aT8);
-    }
-    return (buf, lEN, tRAIL, aT, w256);
-  }
-  proc __m_ilen_write_upto8 (buf:int, lEN:int, w:W64.t) : int * int = {
-    
-    if ((0 < lEN)) {
-      if ((8 <= lEN)) {
-        Glob.mem <- (storeW64 Glob.mem buf w);
-        buf <- (buf + 8);
-        lEN <- (lEN - 8);
-      } else {
-        if ((4 <= lEN)) {
-          Glob.mem <- (storeW32 Glob.mem buf (truncateu32 w));
-          w <- (w `>>` (W8.of_int 32));
-          buf <- (buf + 4);
-          lEN <- (lEN - 4);
-        } else {
-          
-        }
-        if ((2 <= lEN)) {
-          Glob.mem <- (storeW16 Glob.mem buf (truncateu16 w));
-          w <- (w `>>` (W8.of_int 16));
-          buf <- (buf + 2);
-          lEN <- (lEN - 2);
-        } else {
-          
-        }
-        if ((1 <= lEN)) {
-          Glob.mem <- (storeW8 Glob.mem buf (truncateu8 w));
-          buf <- (buf + 1);
-          lEN <- (lEN - 1);
-        } else {
-          
-        }
-      }
-    } else {
-      
-    }
-    return (buf, lEN);
-  }
-  proc __m_ilen_write_upto16 (buf:int, lEN:int, w:W128.t) : int * int = {
-    var t64:W64.t;
-    if ((0 < lEN)) {
-      if ((16 <= lEN)) {
-        Glob.mem <- (storeW128 Glob.mem buf w);
-        buf <- (buf + 16);
-        lEN <- (lEN - 16);
-      } else {
-        if ((8 <= lEN)) {
-          Glob.mem <- (storeW64 Glob.mem buf (MOVV_64 (truncateu64 w)));
-          buf <- (buf + 8);
-          lEN <- (lEN - 8);
-          w <- (VPUNPCKH_2u64 w w);
-        } else {
-          
-        }
-        t64 <- (truncateu64 w);
-        (buf, lEN) <@ __m_ilen_write_upto8 (buf, lEN, t64);
-      }
-    } else {
-      
-    }
-    return (buf, lEN);
-  }
-  proc __m_ilen_write_upto32 (buf:int, lEN:int, w:W256.t) : int * int = {
-    var t128:W128.t;
-    if ((0 < lEN)) {
-      if ((32 <= lEN)) {
-        Glob.mem <- (storeW256 Glob.mem buf w);
-        buf <- (buf + 32);
-        lEN <- (lEN - 32);
-      } else {
-        t128 <- (truncateu128 w);
-        if ((16 <= lEN)) {
-          Glob.mem <- (storeW128 Glob.mem buf t128);
-          buf <- (buf + 16);
-          lEN <- (lEN - 16);
-          t128 <- (VEXTRACTI128 w (W8.of_int 1));
-        } else {
-          
-        }
-        (buf, lEN) <@ __m_ilen_write_upto16 (buf, lEN, t128);
-      }
-    } else {
-      
-    }
-    return (buf, lEN);
-  }
-  proc __m_rlen_read_upto8 (buf:int, len:int) : int * W64.t = {
-    var w:W64.t;
-    var zf:bool;
-    var sh:W8.t;
-    var x:W64.t;
-    var  _0:bool;
-    var  _1:bool;
-    var  _2:bool;
-    var  _3:bool;
-    var  _4:bool;
-    var  _5:bool;
-    var  _6:bool;
-    var  _7:bool;
-    var  _8:bool;
-    var  _9:bool;
-    var  _10:bool;
-    var  _11:bool;
-    if ((8 <= len)) {
-      w <- (loadW64 Glob.mem buf);
-      buf <- (buf + 8);
-    } else {
-      ( _0,  _1,  _2,  _3, zf) <- (TEST_64 (W64.of_int len) (W64.of_int 4));
-      if ((! zf)) {
-        w <- (zeroextu64 (loadW32 Glob.mem buf));
-        buf <- (buf + 4);
-        sh <- (W8.of_int 32);
-      } else {
-        w <- (W64.of_int 0);
-        sh <- (W8.of_int 0);
-      }
-      ( _4,  _5,  _6,  _7, zf) <- (TEST_64 (W64.of_int len) (W64.of_int 2));
-      if ((! zf)) {
-        x <- (zeroextu64 (loadW16 Glob.mem buf));
-        x <- (x `<<` (sh `&` (W8.of_int 63)));
-        w <- (w + x);
-        buf <- (buf + 2);
-        sh <- (sh + (W8.of_int 16));
-      } else {
-        
-      }
-      ( _8,  _9,  _10,  _11, zf) <-
-      (TEST_64 (W64.of_int len) (W64.of_int 1));
-      if ((! zf)) {
-        x <- (zeroextu64 (loadW8 Glob.mem buf));
-        x <- (x `<<` (sh `&` (W8.of_int 63)));
-        w <- (w + x);
-        buf <- (buf + 1);
-      } else {
-        
-      }
-    }
-    return (buf, w);
-  }
-  proc __m_rlen_write_upto8 (buf:int, data:W64.t, len:int) : int = {
-    var zf:bool;
-    var  _0:bool;
-    var  _1:bool;
-    var  _2:bool;
-    var  _3:bool;
-    var  _4:bool;
-    var  _5:bool;
-    var  _6:bool;
-    var  _7:bool;
-    var  _8:bool;
-    var  _9:bool;
-    var  _10:bool;
-    var  _11:bool;
-    if ((8 <= len)) {
-      Glob.mem <- (storeW64 Glob.mem buf data);
-      buf <- (buf + 8);
-    } else {
-      ( _0,  _1,  _2,  _3, zf) <- (TEST_64 (W64.of_int len) (W64.of_int 4));
-      if ((! zf)) {
-        Glob.mem <- (storeW32 Glob.mem buf (truncateu32 data));
-        buf <- (buf + 4);
-        data <- (data `>>` (W8.of_int 32));
-      } else {
-        
-      }
-      ( _4,  _5,  _6,  _7, zf) <- (TEST_64 (W64.of_int len) (W64.of_int 2));
-      if ((! zf)) {
-        Glob.mem <- (storeW16 Glob.mem buf (truncateu16 data));
-        buf <- (buf + 2);
-        data <- (data `>>` (W8.of_int 16));
-      } else {
-        
-      }
-      ( _8,  _9,  _10,  _11, zf) <-
-      (TEST_64 (W64.of_int len) (W64.of_int 1));
-      if ((! zf)) {
-        Glob.mem <- (storeW8 Glob.mem buf (truncateu8 data));
-        buf <- (buf + 1);
-      } else {
-        
-      }
-    }
-    return buf;
-  }
   proc __u64_to_u256 (x:W64.t, l:int) : W256.t = {
     var t256:W256.t;
     var t128:W128.t;
@@ -1921,322 +2099,6 @@ module M = {
       t256 <@ __u64_to_u256 (t64, l);
     }
     st.[r] <- (st.[r] `^` t256);
-    return st;
-  }
-  proc __addstate_m_avx2 (st:W256.t Array7.t, aT:int, buf:int, _LEN:int,
-                          _TRAILB:int) : W256.t Array7.t * int * int = {
-    var t64_1:W64.t;
-    var t128_0:W128.t;
-    var r0:W256.t;
-    var r1:W256.t;
-    var t64_2:W64.t;
-    var t128_1:W128.t;
-    var t128_2:W128.t;
-    var r3:W256.t;
-    var t64_3:W64.t;
-    var r4:W256.t;
-    var t64_4:W64.t;
-    var r5:W256.t;
-    var t64_5:W64.t;
-    var r6:W256.t;
-    var r2:W256.t;
-    if ((aT < 8)) {
-      if (((aT = 0) /\ (8 <= _LEN))) {
-        r0 <- (VPBROADCAST_4u64 (loadW64 Glob.mem buf));
-        buf <- (buf + 8);
-        _LEN <- (_LEN - 8);
-        aT <- 8;
-      } else {
-        (buf, _LEN, _TRAILB, aT, t64_1) <@ __m_ilen_read_upto8_at (buf, 
-        _LEN, _TRAILB, 0, aT);
-        t128_0 <- (zeroextu128 t64_1);
-        r0 <- (VPBROADCAST_4u64 (truncateu64 t128_0));
-      }
-      st.[0] <- (st.[0] `^` r0);
-    } else {
-      
-    }
-    if (((aT < 40) /\ ((0 < _LEN) \/ (_TRAILB <> 0)))) {
-      (buf, _LEN, _TRAILB, aT, r1) <@ __m_ilen_read_upto32_at (buf, _LEN,
-      _TRAILB, 8, aT);
-      st.[1] <- (st.[1] `^` r1);
-    } else {
-      
-    }
-    if (((0 < _LEN) \/ (_TRAILB <> 0))) {
-      (buf, _LEN, _TRAILB, aT, t64_2) <@ __m_ilen_read_upto8_at (buf, 
-      _LEN, _TRAILB, 40, aT);
-      t128_1 <- (zeroextu128 t64_2);
-      t128_2 <- (set0_128);
-      if (((0 < _LEN) \/ (_TRAILB <> 0))) {
-        (buf, _LEN, _TRAILB, aT, r3) <@ __m_ilen_read_upto32_at (buf, 
-        _LEN, _TRAILB, 48, aT);
-        (buf, _LEN, _TRAILB, aT, t64_3) <@ __m_ilen_read_upto8_at (buf, 
-        _LEN, _TRAILB, 80, aT);
-        t128_2 <- (zeroextu128 t64_3);
-        (buf, _LEN, _TRAILB, aT, r4) <@ __m_ilen_read_upto32_at (buf, 
-        _LEN, _TRAILB, 88, aT);
-        (buf, _LEN, _TRAILB, aT, t64_4) <@ __m_ilen_read_upto8_at (buf, 
-        _LEN, _TRAILB, 120, aT);
-        t128_1 <- (VPINSR_2u64 t128_1 t64_4 (W8.of_int 1));
-        (buf, _LEN, _TRAILB, aT, r5) <@ __m_ilen_read_upto32_at (buf, 
-        _LEN, _TRAILB, 128, aT);
-        (buf, _LEN, _TRAILB, aT, t64_5) <@ __m_ilen_read_upto8_at (buf, 
-        _LEN, _TRAILB, 160, aT);
-        t128_2 <- (VPINSR_2u64 t128_2 t64_5 (W8.of_int 1));
-        (buf, _LEN, _TRAILB, aT, r6) <@ __m_ilen_read_upto32_at (buf, 
-        _LEN, _TRAILB, 168, aT);
-        st <@ __addstate_r3456_avx2 (st, r3, r4, r5, r6);
-      } else {
-        
-      }
-      r2 <-
-      (W256.of_int
-      (((W128.to_uint t128_2) %% (2 ^ 128)) +
-      ((2 ^ 128) * (W128.to_uint t128_1))));
-      st.[2] <- (st.[2] `^` r2);
-    } else {
-      
-    }
-    return (st, aT, buf);
-  }
-  proc __absorb_m_avx2 (st:W256.t Array7.t, aT:int, buf:int, _LEN:int,
-                        _TRAILB:int, _RATE8:int) : W256.t Array7.t * int = {
-    var iTERS:int;
-    var i:int;
-    var  _0:int;
-    var  _1:int;
-    var  _2:int;
-    if ((_RATE8 <= (aT + _LEN))) {
-      (st,  _0, buf) <@ __addstate_m_avx2 (st, aT, buf, (_RATE8 - aT), 0);
-      _LEN <- (_LEN - (_RATE8 - aT));
-      aT <- 0;
-      st <@ _keccakf1600_avx2 (st);
-      iTERS <- (_LEN %/ _RATE8);
-      i <- 0;
-      while ((i < iTERS)) {
-        (st,  _1, buf) <@ __addstate_m_avx2 (st, 0, buf, _RATE8, 0);
-        st <@ _keccakf1600_avx2 (st);
-        i <- (i + 1);
-      }
-      _LEN <- (_LEN %% _RATE8);
-    } else {
-      
-    }
-    (st, aT,  _2) <@ __addstate_m_avx2 (st, aT, buf, _LEN, _TRAILB);
-    if ((_TRAILB <> 0)) {
-      st <@ __addratebit_avx2 (st, _RATE8);
-    } else {
-      
-    }
-    return (st, aT);
-  }
-  proc __dumpstate_m_avx2 (buf:int, _LEN:int, st:W256.t Array7.t) : int = {
-    var t128_0:W128.t;
-    var t128_1:W128.t;
-    var t:W64.t;
-    var t256_0:W256.t;
-    var t256_1:W256.t;
-    var t256_2:W256.t;
-    var t256_3:W256.t;
-    var t256_4:W256.t;
-    var  _0:int;
-    if ((8 <= _LEN)) {
-      (buf,  _0) <@ __m_ilen_write_upto32 (buf, 8, st.[0]);
-      _LEN <- (_LEN - 8);
-    } else {
-      (buf, _LEN) <@ __m_ilen_write_upto32 (buf, _LEN, st.[0]);
-    }
-    (buf, _LEN) <@ __m_ilen_write_upto32 (buf, _LEN, st.[1]);
-    if ((0 < _LEN)) {
-      t128_0 <- (truncateu128 st.[2]);
-      t128_1 <- (VEXTRACTI128 st.[2] (W8.of_int 1));
-      t <- (truncateu64 t128_1);
-      (buf, _LEN) <@ __m_ilen_write_upto8 (buf, _LEN, t);
-      t128_1 <- (VPUNPCKH_2u64 t128_1 t128_1);
-      if ((0 < _LEN)) {
-        t256_0 <-
-        (VPBLEND_8u32 st.[3] st.[4]
-        (W8.of_int
-        ((0 %% (2 ^ 1)) +
-        ((2 ^ 1) *
-        ((0 %% (2 ^ 1)) +
-        ((2 ^ 1) *
-        ((0 %% (2 ^ 1)) +
-        ((2 ^ 1) *
-        ((0 %% (2 ^ 1)) +
-        ((2 ^ 1) *
-        ((1 %% (2 ^ 1)) +
-        ((2 ^ 1) *
-        ((1 %% (2 ^ 1)) + ((2 ^ 1) * ((1 %% (2 ^ 1)) + ((2 ^ 1) * 1))))))))))))))
-        ));
-        t256_1 <-
-        (VPBLEND_8u32 st.[4] st.[3]
-        (W8.of_int
-        ((0 %% (2 ^ 1)) +
-        ((2 ^ 1) *
-        ((0 %% (2 ^ 1)) +
-        ((2 ^ 1) *
-        ((0 %% (2 ^ 1)) +
-        ((2 ^ 1) *
-        ((0 %% (2 ^ 1)) +
-        ((2 ^ 1) *
-        ((1 %% (2 ^ 1)) +
-        ((2 ^ 1) *
-        ((1 %% (2 ^ 1)) + ((2 ^ 1) * ((1 %% (2 ^ 1)) + ((2 ^ 1) * 1))))))))))))))
-        ));
-        t256_2 <-
-        (VPBLEND_8u32 st.[5] st.[6]
-        (W8.of_int
-        ((0 %% (2 ^ 1)) +
-        ((2 ^ 1) *
-        ((0 %% (2 ^ 1)) +
-        ((2 ^ 1) *
-        ((0 %% (2 ^ 1)) +
-        ((2 ^ 1) *
-        ((0 %% (2 ^ 1)) +
-        ((2 ^ 1) *
-        ((1 %% (2 ^ 1)) +
-        ((2 ^ 1) *
-        ((1 %% (2 ^ 1)) + ((2 ^ 1) * ((1 %% (2 ^ 1)) + ((2 ^ 1) * 1))))))))))))))
-        ));
-        t256_3 <-
-        (VPBLEND_8u32 st.[6] st.[5]
-        (W8.of_int
-        ((0 %% (2 ^ 1)) +
-        ((2 ^ 1) *
-        ((0 %% (2 ^ 1)) +
-        ((2 ^ 1) *
-        ((0 %% (2 ^ 1)) +
-        ((2 ^ 1) *
-        ((0 %% (2 ^ 1)) +
-        ((2 ^ 1) *
-        ((1 %% (2 ^ 1)) +
-        ((2 ^ 1) *
-        ((1 %% (2 ^ 1)) + ((2 ^ 1) * ((1 %% (2 ^ 1)) + ((2 ^ 1) * 1))))))))))))))
-        ));
-        t256_4 <-
-        (VPBLEND_8u32 t256_0 t256_3
-        (W8.of_int
-        ((1 %% (2 ^ 1)) +
-        ((2 ^ 1) *
-        ((1 %% (2 ^ 1)) +
-        ((2 ^ 1) *
-        ((0 %% (2 ^ 1)) +
-        ((2 ^ 1) *
-        ((0 %% (2 ^ 1)) +
-        ((2 ^ 1) *
-        ((0 %% (2 ^ 1)) +
-        ((2 ^ 1) *
-        ((0 %% (2 ^ 1)) + ((2 ^ 1) * ((1 %% (2 ^ 1)) + ((2 ^ 1) * 1))))))))))))))
-        ));
-        (buf, _LEN) <@ __m_ilen_write_upto32 (buf, _LEN, t256_4);
-        if ((0 < _LEN)) {
-          t <- (truncateu64 t128_0);
-          (buf, _LEN) <@ __m_ilen_write_upto8 (buf, _LEN, t);
-          t128_0 <- (VPUNPCKH_2u64 t128_0 t128_0);
-        } else {
-          
-        }
-        if ((0 < _LEN)) {
-          t256_4 <-
-          (VPBLEND_8u32 t256_3 t256_1
-          (W8.of_int
-          ((1 %% (2 ^ 1)) +
-          ((2 ^ 1) *
-          ((1 %% (2 ^ 1)) +
-          ((2 ^ 1) *
-          ((0 %% (2 ^ 1)) +
-          ((2 ^ 1) *
-          ((0 %% (2 ^ 1)) +
-          ((2 ^ 1) *
-          ((0 %% (2 ^ 1)) +
-          ((2 ^ 1) *
-          ((0 %% (2 ^ 1)) + ((2 ^ 1) * ((1 %% (2 ^ 1)) + ((2 ^ 1) * 1))))))))))))))
-          ));
-          (buf, _LEN) <@ __m_ilen_write_upto32 (buf, _LEN, t256_4);
-        } else {
-          
-        }
-        if ((0 < _LEN)) {
-          t <- (truncateu64 t128_1);
-          (buf, _LEN) <@ __m_ilen_write_upto8 (buf, _LEN, t);
-        } else {
-          
-        }
-        if ((0 < _LEN)) {
-          t256_4 <-
-          (VPBLEND_8u32 t256_2 t256_0
-          (W8.of_int
-          ((1 %% (2 ^ 1)) +
-          ((2 ^ 1) *
-          ((1 %% (2 ^ 1)) +
-          ((2 ^ 1) *
-          ((0 %% (2 ^ 1)) +
-          ((2 ^ 1) *
-          ((0 %% (2 ^ 1)) +
-          ((2 ^ 1) *
-          ((0 %% (2 ^ 1)) +
-          ((2 ^ 1) *
-          ((0 %% (2 ^ 1)) + ((2 ^ 1) * ((1 %% (2 ^ 1)) + ((2 ^ 1) * 1))))))))))))))
-          ));
-          (buf, _LEN) <@ __m_ilen_write_upto32 (buf, _LEN, t256_4);
-        } else {
-          
-        }
-        if ((0 < _LEN)) {
-          t <- (truncateu64 t128_0);
-          (buf, _LEN) <@ __m_ilen_write_upto8 (buf, _LEN, t);
-        } else {
-          
-        }
-        if ((0 < _LEN)) {
-          t256_4 <-
-          (VPBLEND_8u32 t256_1 t256_2
-          (W8.of_int
-          ((1 %% (2 ^ 1)) +
-          ((2 ^ 1) *
-          ((1 %% (2 ^ 1)) +
-          ((2 ^ 1) *
-          ((0 %% (2 ^ 1)) +
-          ((2 ^ 1) *
-          ((0 %% (2 ^ 1)) +
-          ((2 ^ 1) *
-          ((0 %% (2 ^ 1)) +
-          ((2 ^ 1) *
-          ((0 %% (2 ^ 1)) + ((2 ^ 1) * ((1 %% (2 ^ 1)) + ((2 ^ 1) * 1))))))))))))))
-          ));
-          (buf, _LEN) <@ __m_ilen_write_upto32 (buf, _LEN, t256_4);
-        } else {
-          
-        }
-      } else {
-        
-      }
-    } else {
-      
-    }
-    return buf;
-  }
-  proc __squeeze_m_avx2 (st:W256.t Array7.t, buf:int, _LEN:int, _RATE8:int) : 
-  W256.t Array7.t = {
-    var iTERS:int;
-    var lO:int;
-    var i:int;
-    iTERS <- (_LEN %/ _RATE8);
-    lO <- (_LEN %% _RATE8);
-    i <- 0;
-    while ((i < iTERS)) {
-      st <@ _keccakf1600_avx2 (st);
-      buf <@ __dumpstate_m_avx2 (buf, _RATE8, st);
-      i <- (i + 1);
-    }
-    if ((0 < lO)) {
-      st <@ _keccakf1600_avx2 (st);
-      buf <@ __dumpstate_m_avx2 (buf, lO, st);
-    } else {
-      
-    }
     return st;
   }
   proc _keccakf1600_4x_pround (e:W256.t Array25.t, a:W256.t Array25.t,
@@ -2819,371 +2681,6 @@ module M = {
     t256 <- (VPBROADCAST_4u64 (truncateu64 t128));
     t256 <- (t256 `^` st.[((rATE8 - 1) %/ 8)]);
     st.[((rATE8 - 1) %/ 8)] <- t256;
-    return st;
-  }
-  proc __addstate_m_bcast_avx2x4 (st:W256.t Array25.t, aT:int, buf:int,
-                                  _LEN:int, _TRAILB:int) : W256.t Array25.t *
-                                                           int = {
-    var aT8:int;
-    var w:W256.t;
-    var at:int;
-    aT8 <- aT;
-    aT <- (8 * (aT %/ 8));
-    if (((aT8 %% 8) <> 0)) {
-      (buf, _LEN, _TRAILB, aT8, w) <@ __m_ilen_read_bcast_upto8_at (buf,
-      _LEN, _TRAILB, aT, aT8);
-      w <- (w `^` st.[(aT %/ 8)]);
-      st.[(aT %/ 8)] <- w;
-      aT <- aT8;
-    } else {
-      
-    }
-    at <- (32 * (aT %/ 8));
-    while ((at < (32 * ((aT %/ 8) + (_LEN %/ 8))))) {
-      w <- (VPBROADCAST_4u64 (loadW64 Glob.mem buf));
-      buf <- (buf + 8);
-      w <- (w `^` (get256_direct (WArray800.init256 (fun i => st.[i])) at));
-      st <-
-      (Array25.init
-      (WArray800.get256
-      (WArray800.set256_direct (WArray800.init256 (fun i => st.[i])) at w)));
-      at <- (at + 32);
-    }
-    aT <- (aT + (8 * (_LEN %/ 8)));
-    _LEN <- (_LEN %% 8);
-    if (((0 < _LEN) \/ ((_TRAILB %% 256) <> 0))) {
-      (buf, _LEN, _TRAILB, aT, w) <@ __m_ilen_read_bcast_upto8_at (buf, 
-      _LEN, _TRAILB, aT, aT);
-      w <- (w `^` (get256_direct (WArray800.init256 (fun i => st.[i])) at));
-      st <-
-      (Array25.init
-      (WArray800.get256
-      (WArray800.set256_direct (WArray800.init256 (fun i => st.[i])) at w)));
-    } else {
-      
-    }
-    return (st, aT);
-  }
-  proc __absorb_m_bcast_avx2x4 (st:W256.t Array25.t, aT:int, buf:int,
-                                _LEN:int, _TRAILB:int, _RATE8:int) : 
-  W256.t Array25.t * int = {
-    var iTERS:int;
-    var i:int;
-    var  _0:int;
-    var  _1:int;
-    if ((_RATE8 <= (aT + _LEN))) {
-      (st,  _0) <@ __addstate_m_bcast_avx2x4 (st, aT, buf, (_RATE8 - aT), 0);
-      _LEN <- (_LEN - (_RATE8 - aT));
-      aT <- 0;
-      st <@ _keccakf1600_avx2x4 (st);
-      iTERS <- (_LEN %/ _RATE8);
-      i <- 0;
-      while ((i < iTERS)) {
-        (st,  _1) <@ __addstate_m_bcast_avx2x4 (st, 0, buf, _RATE8, 0);
-        st <@ _keccakf1600_avx2x4 (st);
-        i <- (i + 1);
-      }
-      _LEN <- (_LEN %% _RATE8);
-    } else {
-      
-    }
-    (st, aT) <@ __addstate_m_bcast_avx2x4 (st, aT, buf, _LEN, _TRAILB);
-    if ((_TRAILB <> 0)) {
-      st <@ __addratebit_avx2x4 (st, _RATE8);
-    } else {
-      
-    }
-    return (st, aT);
-  }
-  proc __addstate_m_avx2x4 (st:W256.t Array25.t, aT:int, buf0:int, buf1:int,
-                            buf2:int, buf3:int, _LEN:int, _TRAILB:int) : 
-  W256.t Array25.t * int * int * int * int * int = {
-    var aT8:int;
-    var t0:W64.t;
-    var t1:W64.t;
-    var t2:W64.t;
-    var t3:W64.t;
-    var at:int;
-    var  _0:int;
-    var  _1:int;
-    var  _2:int;
-    var  _3:int;
-    var  _4:int;
-    var  _5:int;
-    var  _6:int;
-    var  _7:int;
-    var  _8:int;
-    var  _9:int;
-    var  _10:int;
-    var  _11:int;
-    var  _12:int;
-    var  _13:int;
-    var  _14:int;
-    var  _15:int;
-    var  _16:int;
-    var  _17:int;
-    var  _18:int;
-    var  _19:int;
-    aT8 <- aT;
-    aT <- (8 * (aT %/ 8));
-    if (((aT8 %% 8) <> 0)) {
-      (buf0,  _0,  _1,  _2, t0) <@ __m_ilen_read_upto8_at (buf0, _LEN,
-      _TRAILB, aT, aT8);
-      st <-
-      (Array25.init
-      (WArray800.get256
-      (WArray800.set64 (WArray800.init256 (fun i => st.[i]))
-      ((4 * (aT %/ 8)) + 0)
-      ((get64 (WArray800.init256 (fun i => st.[i])) ((4 * (aT %/ 8)) + 0)) `^`
-      t0))));
-      (buf1,  _3,  _4,  _5, t1) <@ __m_ilen_read_upto8_at (buf1, _LEN,
-      _TRAILB, aT, aT8);
-      st <-
-      (Array25.init
-      (WArray800.get256
-      (WArray800.set64 (WArray800.init256 (fun i => st.[i]))
-      ((4 * (aT %/ 8)) + 1)
-      ((get64 (WArray800.init256 (fun i => st.[i])) ((4 * (aT %/ 8)) + 1)) `^`
-      t1))));
-      (buf2,  _6,  _7,  _8, t2) <@ __m_ilen_read_upto8_at (buf2, _LEN,
-      _TRAILB, aT, aT8);
-      st <-
-      (Array25.init
-      (WArray800.get256
-      (WArray800.set64 (WArray800.init256 (fun i => st.[i]))
-      ((4 * (aT %/ 8)) + 2)
-      ((get64 (WArray800.init256 (fun i => st.[i])) ((4 * (aT %/ 8)) + 2)) `^`
-      t2))));
-      (buf3, _LEN, _TRAILB, aT8, t3) <@ __m_ilen_read_upto8_at (buf3, 
-      _LEN, _TRAILB, aT, aT8);
-      st <-
-      (Array25.init
-      (WArray800.get256
-      (WArray800.set64 (WArray800.init256 (fun i => st.[i]))
-      ((4 * (aT %/ 8)) + 3)
-      ((get64 (WArray800.init256 (fun i => st.[i])) ((4 * (aT %/ 8)) + 3)) `^`
-      t3))));
-      aT <- aT8;
-    } else {
-      
-    }
-    at <- (4 * (aT %/ 8));
-    while ((at < ((4 * (aT %/ 8)) + (4 * (_LEN %/ 8))))) {
-      t0 <- (loadW64 Glob.mem buf0);
-      buf0 <- (buf0 + 8);
-      st <-
-      (Array25.init
-      (WArray800.get256
-      (WArray800.set64 (WArray800.init256 (fun i => st.[i])) (at + 0)
-      ((get64 (WArray800.init256 (fun i => st.[i])) (at + 0)) `^` t0))));
-      t1 <- (loadW64 Glob.mem buf1);
-      buf1 <- (buf1 + 8);
-      st <-
-      (Array25.init
-      (WArray800.get256
-      (WArray800.set64 (WArray800.init256 (fun i => st.[i])) (at + 1)
-      ((get64 (WArray800.init256 (fun i => st.[i])) (at + 1)) `^` t1))));
-      t2 <- (loadW64 Glob.mem buf2);
-      buf2 <- (buf2 + 8);
-      st <-
-      (Array25.init
-      (WArray800.get256
-      (WArray800.set64 (WArray800.init256 (fun i => st.[i])) (at + 2)
-      ((get64 (WArray800.init256 (fun i => st.[i])) (at + 2)) `^` t2))));
-      t3 <- (loadW64 Glob.mem buf3);
-      buf3 <- (buf3 + 8);
-      st <-
-      (Array25.init
-      (WArray800.get256
-      (WArray800.set64 (WArray800.init256 (fun i => st.[i])) (at + 3)
-      ((get64 (WArray800.init256 (fun i => st.[i])) (at + 3)) `^` t3))));
-      at <- (at + 4);
-    }
-    aT <- (aT + (8 * (_LEN %/ 8)));
-    _LEN <- (_LEN %% 8);
-    if (((0 < _LEN) \/ ((_TRAILB %% 256) <> 0))) {
-      (buf0,  _9,  _10,  _11, t0) <@ __m_ilen_read_upto8_at (buf0, _LEN,
-      _TRAILB, aT, aT);
-      st <-
-      (Array25.init
-      (WArray800.get256
-      (WArray800.set64 (WArray800.init256 (fun i => st.[i])) (at + 0)
-      ((get64 (WArray800.init256 (fun i => st.[i])) (at + 0)) `^` t0))));
-      (buf1,  _12,  _13,  _14, t1) <@ __m_ilen_read_upto8_at (buf1, _LEN,
-      _TRAILB, aT, aT);
-      st <-
-      (Array25.init
-      (WArray800.get256
-      (WArray800.set64 (WArray800.init256 (fun i => st.[i])) (at + 1)
-      ((get64 (WArray800.init256 (fun i => st.[i])) (at + 1)) `^` t1))));
-      (buf2,  _15,  _16,  _17, t2) <@ __m_ilen_read_upto8_at (buf2, _LEN,
-      _TRAILB, aT, aT);
-      st <-
-      (Array25.init
-      (WArray800.get256
-      (WArray800.set64 (WArray800.init256 (fun i => st.[i])) (at + 2)
-      ((get64 (WArray800.init256 (fun i => st.[i])) (at + 2)) `^` t2))));
-      (buf3,  _18,  _19, aT, t3) <@ __m_ilen_read_upto8_at (buf3, _LEN,
-      _TRAILB, aT, aT);
-      st <-
-      (Array25.init
-      (WArray800.get256
-      (WArray800.set64 (WArray800.init256 (fun i => st.[i])) (at + 3)
-      ((get64 (WArray800.init256 (fun i => st.[i])) (at + 3)) `^` t3))));
-    } else {
-      
-    }
-    return (st, aT, buf0, buf1, buf2, buf3);
-  }
-  proc __absorb_m_avx2x4 (st:W256.t Array25.t, aT:int, buf0:int, buf1:int,
-                          buf2:int, buf3:int, _LEN:int, _TRAILB:int,
-                          _RATE8:int) : W256.t Array25.t * int = {
-    var iTERS:int;
-    var i:int;
-    var  _0:int;
-    var  _1:int;
-    var  _2:int;
-    var  _3:int;
-    var  _4:int;
-    var  _5:int;
-    if ((_RATE8 <= (aT + _LEN))) {
-      (st,  _0, buf0, buf1, buf2, buf3) <@ __addstate_m_avx2x4 (st, aT, 
-      buf0, buf1, buf2, buf3, (_RATE8 - aT), 0);
-      _LEN <- (_LEN - (_RATE8 - aT));
-      aT <- 0;
-      st <@ _keccakf1600_avx2x4 (st);
-      iTERS <- (_LEN %/ _RATE8);
-      i <- 0;
-      while ((i < iTERS)) {
-        (st,  _1, buf0, buf1, buf2, buf3) <@ __addstate_m_avx2x4 (st, 0,
-        buf0, buf1, buf2, buf3, _RATE8, 0);
-        st <@ _keccakf1600_avx2x4 (st);
-        i <- (i + 1);
-      }
-      _LEN <- (_LEN %% _RATE8);
-    } else {
-      
-    }
-    (st, aT,  _2,  _3,  _4,  _5) <@ __addstate_m_avx2x4 (st, aT, buf0, 
-    buf1, buf2, buf3, _LEN, _TRAILB);
-    if ((_TRAILB <> 0)) {
-      st <@ __addratebit_avx2x4 (st, _RATE8);
-    } else {
-      
-    }
-    return (st, aT);
-  }
-  proc __dumpstate_m_avx2x4 (buf0:int, buf1:int, buf2:int, buf3:int,
-                             _LEN:int, st:W256.t Array25.t) : int * int *
-                                                              int * int = {
-    var x0:W256.t;
-    var x1:W256.t;
-    var x2:W256.t;
-    var x3:W256.t;
-    var t0:W64.t;
-    var t1:W64.t;
-    var t2:W64.t;
-    var t3:W64.t;
-    var i:int;
-    var  _0:int;
-    var  _1:int;
-    var  _2:int;
-    var  _3:int;
-    i <- 0;
-    while ((i < (32 * (_LEN %/ 32)))) {
-      x0 <-
-      (get256_direct (WArray800.init256 (fun i_0 => st.[i_0]))
-      ((4 * i) + (0 * 32)));
-      x1 <-
-      (get256_direct (WArray800.init256 (fun i_0 => st.[i_0]))
-      ((4 * i) + (1 * 32)));
-      x2 <-
-      (get256_direct (WArray800.init256 (fun i_0 => st.[i_0]))
-      ((4 * i) + (2 * 32)));
-      x3 <-
-      (get256_direct (WArray800.init256 (fun i_0 => st.[i_0]))
-      ((4 * i) + (3 * 32)));
-      i <- (i + 32);
-      (x0, x1, x2, x3) <@ __4u64x4_u256x4 (x0, x1, x2, x3);
-      Glob.mem <- (storeW256 Glob.mem buf0 x0);
-      buf0 <- (buf0 + 32);
-      Glob.mem <- (storeW256 Glob.mem buf1 x1);
-      buf1 <- (buf1 + 32);
-      Glob.mem <- (storeW256 Glob.mem buf2 x2);
-      buf2 <- (buf2 + 32);
-      Glob.mem <- (storeW256 Glob.mem buf3 x3);
-      buf3 <- (buf3 + 32);
-    }
-    while ((i < (8 * (_LEN %/ 8)))) {
-      t0 <-
-      (get64_direct (WArray800.init256 (fun i_0 => st.[i_0]))
-      ((4 * i) + (0 * 8)));
-      Glob.mem <- (storeW64 Glob.mem (buf0 + i) t0);
-      t1 <-
-      (get64_direct (WArray800.init256 (fun i_0 => st.[i_0]))
-      ((4 * i) + (1 * 8)));
-      Glob.mem <- (storeW64 Glob.mem (buf1 + i) t1);
-      t2 <-
-      (get64_direct (WArray800.init256 (fun i_0 => st.[i_0]))
-      ((4 * i) + (2 * 8)));
-      Glob.mem <- (storeW64 Glob.mem (buf2 + i) t2);
-      t3 <-
-      (get64_direct (WArray800.init256 (fun i_0 => st.[i_0]))
-      ((4 * i) + (3 * 8)));
-      Glob.mem <- (storeW64 Glob.mem (buf3 + i) t3);
-      i <- (i + 8);
-    }
-    buf0 <- (buf0 + i);
-    buf1 <- (buf1 + i);
-    buf2 <- (buf2 + i);
-    buf3 <- (buf3 + i);
-    if ((0 < (_LEN %% 8))) {
-      t0 <-
-      (get64_direct (WArray800.init256 (fun i_0 => st.[i_0]))
-      ((4 * i) + (0 * 8)));
-      (buf0,  _0) <@ __m_ilen_write_upto8 (buf0, (_LEN %% 8), t0);
-      t1 <-
-      (get64_direct (WArray800.init256 (fun i_0 => st.[i_0]))
-      ((4 * i) + (1 * 8)));
-      (buf1,  _1) <@ __m_ilen_write_upto8 (buf1, (_LEN %% 8), t1);
-      t2 <-
-      (get64_direct (WArray800.init256 (fun i_0 => st.[i_0]))
-      ((4 * i) + (2 * 8)));
-      (buf2,  _2) <@ __m_ilen_write_upto8 (buf2, (_LEN %% 8), t2);
-      t3 <-
-      (get64_direct (WArray800.init256 (fun i_0 => st.[i_0]))
-      ((4 * i) + (3 * 8)));
-      (buf3,  _3) <@ __m_ilen_write_upto8 (buf3, (_LEN %% 8), t3);
-    } else {
-      
-    }
-    return (buf0, buf1, buf2, buf3);
-  }
-  proc __squeeze_m_avx2x4 (st:W256.t Array25.t, buf0:int, buf1:int, buf2:int,
-                           buf3:int, _LEN:int, _RATE8:int) : W256.t Array25.t = {
-    var iTERS:int;
-    var lO:int;
-    var i:int;
-    iTERS <- (_LEN %/ _RATE8);
-    lO <- (_LEN %% _RATE8);
-    if ((0 < iTERS)) {
-      i <- 0;
-      while ((i < iTERS)) {
-        st <@ _keccakf1600_avx2x4 (st);
-        (buf0, buf1, buf2, buf3) <@ __dumpstate_m_avx2x4 (buf0, buf1, 
-        buf2, buf3, _RATE8, st);
-        i <- (i + 1);
-      }
-    } else {
-      
-    }
-    if ((0 < lO)) {
-      st <@ _keccakf1600_avx2x4 (st);
-      (buf0, buf1, buf2, buf3) <@ __dumpstate_m_avx2x4 (buf0, buf1, buf2,
-      buf3, lO, st);
-    } else {
-      
-    }
     return st;
   }
   proc __a_ilen_read_upto8_at (buf:W8.t Array999.t, offset:int, dELTA:int,
@@ -3905,6 +3402,135 @@ module M = {
       
     }
     return (buf, dELTA, lEN);
+  }
+  proc __addstate_ref (st:W64.t Array25.t, aT:int, buf:W8.t Array999.t,
+                       offset:int, _LEN:int, _TRAILB:int) : W64.t Array25.t *
+                                                            int * int = {
+    var dELTA:int;
+    var aT8:int;
+    var w:W64.t;
+    var at:int;
+    dELTA <- 0;
+    aT8 <- aT;
+    aT <- (8 * (aT %/ 8));
+    if ((aT8 <> 0)) {
+      (dELTA, _LEN, _TRAILB, aT8, w) <@ __a_ilen_read_upto8_at (buf, 
+      offset, dELTA, _LEN, _TRAILB, aT, aT8);
+      st.[(aT %/ 8)] <- (st.[(aT %/ 8)] `^` w);
+      aT <- aT8;
+    } else {
+      
+    }
+    offset <- (offset + dELTA);
+    at <- (aT %/ 8);
+    while ((at < ((aT %/ 8) + (_LEN %/ 8)))) {
+      w <- (get64_direct (WArray999.init8 (fun i => buf.[i])) offset);
+      offset <- (offset + 8);
+      st.[at] <- (st.[at] `^` w);
+      at <- (at + 1);
+    }
+    aT <- (aT + (8 * (_LEN %/ 8)));
+    _LEN <- (_LEN %% 8);
+    if (((0 < _LEN) \/ ((_TRAILB %% 256) <> 0))) {
+      (dELTA, _LEN, _TRAILB, aT, w) <@ __a_ilen_read_upto8_at (buf, offset,
+      0, _LEN, _TRAILB, aT, aT);
+      st.[at] <- (st.[at] `^` w);
+      offset <- (offset + dELTA);
+    } else {
+      
+    }
+    return (st, aT, offset);
+  }
+  proc __absorb_ref (st:W64.t Array25.t, aT:int, buf:W8.t Array999.t,
+                     _TRAILB:int, _RATE8:int) : W64.t Array25.t * int = {
+    var _LEN:int;
+    var iTERS:int;
+    var offset:int;
+    var i:int;
+    var  _0:int;
+    var  _1:int;
+    var  _2:int;
+    offset <- 0;
+    _LEN <- 999;
+    if ((_RATE8 <= (aT + _LEN))) {
+      (st,  _0, offset) <@ __addstate_ref (st, aT, buf, offset,
+      (_RATE8 - aT), 0);
+      _LEN <- (_LEN - (_RATE8 - aT));
+      aT <- 0;
+      (* Erased call to spill *)
+      st <@ _keccakf1600_ref (st);
+      (* Erased call to unspill *)
+      iTERS <- (_LEN %/ _RATE8);
+      i <- 0;
+      while ((i < iTERS)) {
+        (st,  _1, offset) <@ __addstate_ref (st, 0, buf, offset, _RATE8, 0);
+        (* Erased call to spill *)
+        st <@ _keccakf1600_ref (st);
+        (* Erased call to unspill *)
+        i <- (i + 1);
+      }
+      _LEN <- (_LEN %% _RATE8);
+    } else {
+      
+    }
+    (st, aT,  _2) <@ __addstate_ref (st, aT, buf, offset, _LEN, _TRAILB);
+    if ((_TRAILB <> 0)) {
+      st <@ __addratebit_ref (st, _RATE8);
+    } else {
+      
+    }
+    return (st, aT);
+  }
+  proc __dumpstate_ref (buf:W8.t Array999.t, offset:int, _LEN:int,
+                        st:W64.t Array25.t) : W8.t Array999.t * int = {
+    var t:W64.t;
+    var dELTA:int;
+    var i:int;
+    var  _0:int;
+    i <- 0;
+    while ((i < (_LEN %/ 8))) {
+      t <- st.[i];
+      buf <-
+      (Array999.init
+      (WArray999.get8
+      (WArray999.set64_direct (WArray999.init8 (fun i_0 => buf.[i_0])) 
+      offset t)));
+      offset <- (offset + 8);
+      i <- (i + 1);
+    }
+    if ((0 < (_LEN %% 8))) {
+      t <- st.[i];
+      (buf, dELTA,  _0) <@ __a_ilen_write_upto8 (buf, offset, 0, (_LEN %% 8),
+      t);
+      offset <- (offset + dELTA);
+    } else {
+      
+    }
+    return (buf, offset);
+  }
+  proc __squeeze_ref (st:W64.t Array25.t, buf:W8.t Array999.t, _RATE8:int) : 
+  W64.t Array25.t * W8.t Array999.t = {
+    var offset:int;
+    var i:int;
+    offset <- 0;
+    i <- 0;
+    while ((i < (999 %/ _RATE8))) {
+      (* Erased call to spill *)
+      st <@ _keccakf1600_ref (st);
+      (* Erased call to unspill *)
+      (buf, offset) <@ __dumpstate_ref (buf, offset, _RATE8, st);
+      (* Erased call to unspill *)
+      i <- (i + 1);
+    }
+    if ((0 < (999 %% _RATE8))) {
+      (* Erased call to spill *)
+      st <@ _keccakf1600_ref (st);
+      (* Erased call to unspill *)
+      (buf, offset) <@ __dumpstate_ref (buf, offset, (999 %% _RATE8), st);
+    } else {
+      
+    }
+    return (st, buf);
   }
   proc __addstate_avx2 (st:W256.t Array7.t, aT:int, buf:W8.t Array999.t,
                         offset:int, _LEN:int, _TRAILB:int) : W256.t Array7.t *
