proof/amd64/avx2/Keccak1600_fixedsizes_avx2.ec
@@ -1,0 +1,655 @@
+(******************************************************************************
+   avx2/Keccak1600_fixedsizes.ec:
+
+   Correctness proof for the Keccak (fixed-sized) memory and array 
+  absorb/squeeze AVX2 implementation
+
+******************************************************************************)
+
+require import AllCore List Int IntDiv.
+
+from Jasmin require import JModel_x86.
+
+from JazzEC require import Keccak1600_Jazz.
+from JazzEC require import WArray200.
+from JazzEC require import Array7 Array25.
+
+from CryptoSpecs require import JWordList.
+from CryptoSpecs require import FIPS202_Keccakf1600.
+from CryptoSpecs require import FIPS202_SHA3_Spec Keccakf1600_Spec Keccak1600_Spec.
+
+
+require export Keccak1600_avx2 Keccakf1600_avx2.
+require import Keccak1600_subreadwrite.
+
+(*
+   INCREMENTAL (FIXED-SIZE) MEMORY ABSORB
+   ======================================
+*)
+
+lemma addstate_m_avx2_ll: islossless M.__addstate_m_avx2
+ by islossless.
+
+lemma absorb_m_avx2_ll: islossless M.__absorb_m_avx2.
+proof.
+proc.
+seq 2: true => //=; last first.
+ if => //.
+ by call addratebit_avx2_ll.
+call addstate_m_avx2_ll.
+if => //.
+ wp; while true (iTERS-i).
+ move=> z; wp.
+ call keccakf1600_avx2_ll.
+ call addstate_m_avx2_ll.
+ by auto => /#.
+wp; call keccakf1600_avx2_ll.
+wp; call addstate_m_avx2_ll.
+by auto => /#.
+qed.
+
+require BitEncoding.
+import BitEncoding.BitChunking.
+
+
+op pabsorb_spec_avx2 (r8 : int) (l : W8.t list) (st : W256.t Array7.t) : bool =
+  0 < r8 <= 200 /\
+  st = stavx2_from_st25 
+        (addstate
+          (stateabsorb_iblocks (chunk r8 l) st0)
+          (bytes2state (chunkremains r8 l))).
+
+
+hoare absorb_m_avx2_h _mem _l _buf _len _r8 _tb:
+ M.__absorb_m_avx2
+ : Glob.mem=_mem /\ aT = size _l %% _r8 /\ buf=_buf /\ _LEN=_len /\ _RATE8=_r8 /\ _TRAILB=_tb
+ /\ pabsorb_spec_avx2 _r8 _l st
+ /\ 0 <= _len
+ /\ _buf + _len < W64.modulus
+ ==> if _tb <> 0
+     then absorb_spec_avx2 _r8 _tb (_l ++ memread _mem _buf _len) res.`1
+     else pabsorb_spec_avx2 _r8 (_l ++ memread _mem _buf _len) res.`1
+          /\ res.`2 = (size _l + _len) %% _r8.
+proof.
+proc => /=.
+admitted.
+
+phoare absorb_m_avx2_ph _mem _l _buf _len _r8 _tb:
+ [ M.__absorb_m_avx2
+ : Glob.mem=_mem /\ aT = size _l %% _r8 /\ buf=_buf /\ _LEN=_len /\ _RATE8=_r8 /\ _TRAILB=_tb
+ /\ pabsorb_spec_avx2 _r8 _l st
+ /\ 0 <= _len
+ /\ _buf + _len < W64.modulus
+ ==> if _tb <> 0
+     then absorb_spec_avx2 _r8 _tb (_l ++ memread _mem _buf _len) res.`1
+     else pabsorb_spec_avx2 _r8 (_l ++ memread _mem _buf _len) res.`1
+          /\ res.`2 = (size _l + _len) %% _r8
+ ] = 1%r.
+proof.
+by conseq absorb_m_avx2_ll (absorb_m_avx2_h _mem _l _buf _len _r8 _tb).
+qed.
+
+(*
+   ONE-SHOT (FIXED-SIZE) MEMORY SQUEEZE
+   ====================================
+*)
+
+lemma dumpstate_m_avx2_ll: islossless M.__dumpstate_m_avx2
+ by islossless.
+
+hoare dumpstate_m_avx2_h _mem _buf _len _st:
+ M.__dumpstate_m_avx2
+ : Glob.mem=_mem /\ buf=_buf /\ _LEN=_len /\ st=_st
+ /\ 0 <= _len <= 200
+ /\ _buf + _len < W64.modulus
+ ==> Glob.mem = stores _mem _buf (sub (stbytes (stavx2_to_st25 _st)) 0 _len)
+  /\ res = _buf + _len.
+proof.
+proc => /=.
+admitted.
+
+phoare dumpstate_m_avx2_ph _mem _buf _len _st:
+ [ M.__dumpstate_m_avx2
+ : Glob.mem=_mem /\ buf=_buf /\ _LEN=_len /\ st=_st
+ /\ 0 <= _len <= 200
+ /\ _buf + _len < W64.modulus
+ ==> Glob.mem = stores _mem _buf (sub (stbytes (stavx2_to_st25 _st)) 0 _len)
+  /\ res = _buf + _len
+ ] = 1%r.
+proof.
+by conseq dumpstate_m_avx2_ll (dumpstate_m_avx2_h _mem _buf _len _st).
+qed.
+
+lemma squeeze_m_avx2_ll: islossless M.__squeeze_m_avx2.
+proof.
+proc.
+seq 4: true => //.
+ while true (iTERS-i).
+  move=> z.
+  wp; call dumpstate_m_avx2_ll.
+  call keccakf1600_avx2_ll.
+  by auto => /#.
+ auto => /#.
+if => //.
+call dumpstate_m_avx2_ll.
+call keccakf1600_avx2_ll.
+by auto.
+qed.
+
+hoare squeeze_m_avx2_h _mem _buf _len _st _r8:
+ M.__squeeze_m_avx2
+ : Glob.mem=_mem /\ buf=_buf /\ _LEN=_len /\ st=_st /\ _RATE8=_r8
+ /\ 0 <= _len
+ /\ 0 < _r8 <= 200
+ /\ _buf + _len < W64.modulus
+ ==> Glob.mem = stores _mem _buf (SQUEEZE1600 _r8 _len (stavx2_to_st25 _st))
+  /\ res = stavx2_from_st25 (st_i (stavx2_to_st25 _st) ((_len-1) %/ _r8 + 1)).
+proof.
+proc.
+admitted.
+
+phoare squeeze_m_avx2_ph _mem _buf _len _st _r8:
+ [ M.__squeeze_m_avx2
+ : Glob.mem=_mem /\ buf=_buf /\ _LEN=_len /\ st=_st /\ _RATE8=_r8
+ /\ 0 <= _len
+ /\ 0 < _r8 <= 200
+ /\ _buf + _len < W64.modulus
+ ==> Glob.mem = stores _mem _buf (SQUEEZE1600 _r8 _len (stavx2_to_st25 _st))
+  /\ res = stavx2_from_st25 (st_i (stavx2_to_st25 _st) ((_len-1) %/ _r8 + 1))
+ ] = 1%r.
+proof.
+by conseq squeeze_m_avx2_ll (squeeze_m_avx2_h _mem _buf _len _st _r8).
+qed.
+
+
+
+abstract theory KeccakArrayAvx2.
+
+op _ASIZE: int.
+
+axiom _ASIZE_ge0: 0 <= _ASIZE.
+axiom _ASIZE_u64: _ASIZE < W64.modulus.
+
+clone import PolyArray as A
+ with op size <- _ASIZE
+      proof ge0_size by exact _ASIZE_ge0.
+
+clone import WArray as WA
+ with op size <- _ASIZE.
+
+clone import ReadWriteArray as RW
+ with op _ASIZE <- _ASIZE,
+      theory A <- A,
+      theory WA <- WA
+      proof _ASIZE_ge0 by exact _ASIZE_ge0
+      proof _ASIZE_u64 by exact _ASIZE_u64.
+
+
+module MM = {
+  proc __addstate_avx2 (st:W256.t Array7.t, aT:int, buf:W8.t A.t,
+                        offset:int, _LEN:int, _TRAILB:int) : W256.t Array7.t *
+                                                             int * int = {
+    var dELTA:int;
+    var t64_1:W64.t;
+    var t128_0:W128.t;
+    var r0:W256.t;
+    var r1:W256.t;
+    var t64_2:W64.t;
+    var t128_1:W128.t;
+    var t128_2:W128.t;
+    var r3:W256.t;
+    var t64_3:W64.t;
+    var r4:W256.t;
+    var t64_4:W64.t;
+    var r5:W256.t;
+    var t64_5:W64.t;
+    var r6:W256.t;
+    var r2:W256.t;
+    dELTA <- 0;
+    if ((aT < 8)) {
+      if (((aT = 0) /\ (8 <= _LEN))) {
+        r0 <-
+        (VPBROADCAST_4u64
+        (get64_direct (WA.init8 (fun i => buf.[i]))
+        (W64.to_uint ((W64.of_int offset) + (W64.of_int dELTA)))));
+        dELTA <- (dELTA + 8);
+        _LEN <- (_LEN - 8);
+        aT <- 8;
+      } else {
+        (dELTA, _LEN, _TRAILB, aT, t64_1) <@ RW.MM.__a_ilen_read_upto8_at (
+        buf, offset, dELTA, _LEN, _TRAILB, 0, aT);
+        t128_0 <- (zeroextu128 t64_1);
+        r0 <- (VPBROADCAST_4u64 (truncateu64 t128_0));
+      }
+      st.[0] <- (st.[0] `^` r0);
+    } else {
+      
+    }
+    if (((aT < 40) /\ ((0 < _LEN) \/ (_TRAILB <> 0)))) {
+      (dELTA, _LEN, _TRAILB, aT, r1) <@ RW.MM.__a_ilen_read_upto32_at (buf, 
+      offset, dELTA, _LEN, _TRAILB, 8, aT);
+      st.[1] <- (st.[1] `^` r1);
+    } else {
+      
+    }
+    if (((0 < _LEN) \/ (_TRAILB <> 0))) {
+      (dELTA, _LEN, _TRAILB, aT, t64_2) <@ RW.MM.__a_ilen_read_upto8_at (buf,
+      offset, dELTA, _LEN, _TRAILB, 40, aT);
+      t128_1 <- (zeroextu128 t64_2);
+      t128_2 <- (set0_128);
+      if (((0 < _LEN) \/ (_TRAILB <> 0))) {
+        (dELTA, _LEN, _TRAILB, aT, r3) <@ RW.MM.__a_ilen_read_upto32_at (buf,
+        offset, dELTA, _LEN, _TRAILB, 48, aT);
+        (dELTA, _LEN, _TRAILB, aT, t64_3) <@ RW.MM.__a_ilen_read_upto8_at (
+        buf, offset, dELTA, _LEN, _TRAILB, 80, aT);
+        t128_2 <- (zeroextu128 t64_3);
+        (dELTA, _LEN, _TRAILB, aT, r4) <@ RW.MM.__a_ilen_read_upto32_at (buf,
+        offset, dELTA, _LEN, _TRAILB, 88, aT);
+        (dELTA, _LEN, _TRAILB, aT, t64_4) <@ RW.MM.__a_ilen_read_upto8_at (
+        buf, offset, dELTA, _LEN, _TRAILB, 120, aT);
+        t128_1 <- (VPINSR_2u64 t128_1 t64_4 (W8.of_int 1));
+        (dELTA, _LEN, _TRAILB, aT, r5) <@ RW.MM.__a_ilen_read_upto32_at (buf,
+        offset, dELTA, _LEN, _TRAILB, 128, aT);
+        (dELTA, _LEN, _TRAILB, aT, t64_5) <@ RW.MM.__a_ilen_read_upto8_at (
+        buf, offset, dELTA, _LEN, _TRAILB, 160, aT);
+        t128_2 <- (VPINSR_2u64 t128_2 t64_5 (W8.of_int 1));
+        (dELTA, _LEN, _TRAILB, aT, r6) <@ RW.MM.__a_ilen_read_upto32_at (buf,
+        offset, dELTA, _LEN, _TRAILB, 168, aT);
+        st <@ M.__addstate_r3456_avx2 (st, r3, r4, r5, r6);
+      } else {
+        
+      }
+      r2 <-
+      (W256.of_int
+      (((W128.to_uint t128_2) %% (2 ^ 128)) +
+      ((2 ^ 128) * (W128.to_uint t128_1))));
+      st.[2] <- (st.[2] `^` r2);
+    } else {
+      
+    }
+    offset <- (offset + dELTA);
+    return (st, aT, offset);
+  }
+  proc __absorb_avx2 (st:W256.t Array7.t, aT:int, buf:W8.t A.t,
+                      _TRAILB:int, _RATE8:int) : W256.t Array7.t * int = {
+    var _LEN:int;
+    var iTERS:int;
+    var offset:int;
+    var i:int;
+    var  _0:int;
+    var  _1:int;
+    var  _2:int;
+    offset <- 0;
+    _LEN <- _ASIZE;
+    if ((_RATE8 <= (aT + _LEN))) {
+      (st,  _0, offset) <@ __addstate_avx2 (st, aT, buf, offset,
+      (_RATE8 - aT), 0);
+      _LEN <- (_LEN - (_RATE8 - aT));
+      aT <- 0;
+      st <@ M._keccakf1600_avx2 (st);
+      iTERS <- (_LEN %/ _RATE8);
+      i <- 0;
+      while ((i < iTERS)) {
+        (st,  _1, offset) <@ __addstate_avx2 (st, 0, buf, offset, _RATE8, 0);
+        st <@ M._keccakf1600_avx2 (st);
+        i <- (i + 1);
+      }
+      _LEN <- (_LEN %% _RATE8);
+    } else {
+      
+    }
+    (st, aT,  _2) <@ __addstate_avx2 (st, aT, buf, offset, _LEN, _TRAILB);
+    if ((_TRAILB <> 0)) {
+      st <@ M.__addratebit_avx2 (st, _RATE8);
+    } else {
+      
+    }
+    return (st, aT);
+  }
+  proc __dumpstate_avx2 (buf:W8.t A.t, offset:int, _LEN:int,
+                         st:W256.t Array7.t) : W8.t A.t * int = {
+    var dELTA:int;
+    var t128_0:W128.t;
+    var t128_1:W128.t;
+    var t:W64.t;
+    var t256_0:W256.t;
+    var t256_1:W256.t;
+    var t256_2:W256.t;
+    var t256_3:W256.t;
+    var t256_4:W256.t;
+    var  _0:int;
+    dELTA <- 0;
+    if ((8 <= _LEN)) {
+      (buf, dELTA,  _0) <@ RW.MM.__a_ilen_write_upto32 (buf, offset, dELTA, 8,
+      st.[0]);
+      _LEN <- (_LEN - 8);
+    } else {
+      (buf, dELTA, _LEN) <@ RW.MM.__a_ilen_write_upto32 (buf, offset, dELTA, 
+      _LEN, st.[0]);
+    }
+    (buf, dELTA, _LEN) <@ RW.MM.__a_ilen_write_upto32 (buf, offset, dELTA, 
+    _LEN, st.[1]);
+    if ((0 < _LEN)) {
+      t128_0 <- (truncateu128 st.[2]);
+      t128_1 <- (VEXTRACTI128 st.[2] (W8.of_int 1));
+      t <- (truncateu64 t128_1);
+      (buf, dELTA, _LEN) <@ RW.MM.__a_ilen_write_upto8 (buf, offset, dELTA, 
+      _LEN, t);
+      t128_1 <- (VPUNPCKH_2u64 t128_1 t128_1);
+      if ((0 < _LEN)) {
+        t256_0 <-
+        (VPBLEND_8u32 st.[3] st.[4]
+        (W8.of_int
+        ((0 %% (2 ^ 1)) +
+        ((2 ^ 1) *
+        ((0 %% (2 ^ 1)) +
+        ((2 ^ 1) *
+        ((0 %% (2 ^ 1)) +
+        ((2 ^ 1) *
+        ((0 %% (2 ^ 1)) +
+        ((2 ^ 1) *
+        ((1 %% (2 ^ 1)) +
+        ((2 ^ 1) *
+        ((1 %% (2 ^ 1)) + ((2 ^ 1) * ((1 %% (2 ^ 1)) + ((2 ^ 1) * 1))))))))))))))
+        ));
+        t256_1 <-
+        (VPBLEND_8u32 st.[4] st.[3]
+        (W8.of_int
+        ((0 %% (2 ^ 1)) +
+        ((2 ^ 1) *
+        ((0 %% (2 ^ 1)) +
+        ((2 ^ 1) *
+        ((0 %% (2 ^ 1)) +
+        ((2 ^ 1) *
+        ((0 %% (2 ^ 1)) +
+        ((2 ^ 1) *
+        ((1 %% (2 ^ 1)) +
+        ((2 ^ 1) *
+        ((1 %% (2 ^ 1)) + ((2 ^ 1) * ((1 %% (2 ^ 1)) + ((2 ^ 1) * 1))))))))))))))
+        ));
+        t256_2 <-
+        (VPBLEND_8u32 st.[5] st.[6]
+        (W8.of_int
+        ((0 %% (2 ^ 1)) +
+        ((2 ^ 1) *
+        ((0 %% (2 ^ 1)) +
+        ((2 ^ 1) *
+        ((0 %% (2 ^ 1)) +
+        ((2 ^ 1) *
+        ((0 %% (2 ^ 1)) +
+        ((2 ^ 1) *
+        ((1 %% (2 ^ 1)) +
+        ((2 ^ 1) *
+        ((1 %% (2 ^ 1)) + ((2 ^ 1) * ((1 %% (2 ^ 1)) + ((2 ^ 1) * 1))))))))))))))
+        ));
+        t256_3 <-
+        (VPBLEND_8u32 st.[6] st.[5]
+        (W8.of_int
+        ((0 %% (2 ^ 1)) +
+        ((2 ^ 1) *
+        ((0 %% (2 ^ 1)) +
+        ((2 ^ 1) *
+        ((0 %% (2 ^ 1)) +
+        ((2 ^ 1) *
+        ((0 %% (2 ^ 1)) +
+        ((2 ^ 1) *
+        ((1 %% (2 ^ 1)) +
+        ((2 ^ 1) *
+        ((1 %% (2 ^ 1)) + ((2 ^ 1) * ((1 %% (2 ^ 1)) + ((2 ^ 1) * 1))))))))))))))
+        ));
+        t256_4 <-
+        (VPBLEND_8u32 t256_0 t256_3
+        (W8.of_int
+        ((1 %% (2 ^ 1)) +
+        ((2 ^ 1) *
+        ((1 %% (2 ^ 1)) +
+        ((2 ^ 1) *
+        ((0 %% (2 ^ 1)) +
+        ((2 ^ 1) *
+        ((0 %% (2 ^ 1)) +
+        ((2 ^ 1) *
+        ((0 %% (2 ^ 1)) +
+        ((2 ^ 1) *
+        ((0 %% (2 ^ 1)) + ((2 ^ 1) * ((1 %% (2 ^ 1)) + ((2 ^ 1) * 1))))))))))))))
+        ));
+        (buf, dELTA, _LEN) <@ RW.MM.__a_ilen_write_upto32 (buf, offset, dELTA,
+        _LEN, t256_4);
+        if ((0 < _LEN)) {
+          t <- (truncateu64 t128_0);
+          (buf, dELTA, _LEN) <@ RW.MM.__a_ilen_write_upto8 (buf, offset, dELTA,
+          _LEN, t);
+          t128_0 <- (VPUNPCKH_2u64 t128_0 t128_0);
+        } else {
+          
+        }
+        if ((0 < _LEN)) {
+          t256_4 <-
+          (VPBLEND_8u32 t256_3 t256_1
+          (W8.of_int
+          ((1 %% (2 ^ 1)) +
+          ((2 ^ 1) *
+          ((1 %% (2 ^ 1)) +
+          ((2 ^ 1) *
+          ((0 %% (2 ^ 1)) +
+          ((2 ^ 1) *
+          ((0 %% (2 ^ 1)) +
+          ((2 ^ 1) *
+          ((0 %% (2 ^ 1)) +
+          ((2 ^ 1) *
+          ((0 %% (2 ^ 1)) + ((2 ^ 1) * ((1 %% (2 ^ 1)) + ((2 ^ 1) * 1))))))))))))))
+          ));
+          (buf, dELTA, _LEN) <@ RW.MM.__a_ilen_write_upto32 (buf, offset, dELTA,
+          _LEN, t256_4);
+        } else {
+          
+        }
+        if ((0 < _LEN)) {
+          t <- (truncateu64 t128_1);
+          (buf, dELTA, _LEN) <@ RW.MM.__a_ilen_write_upto8 (buf, offset, dELTA,
+          _LEN, t);
+        } else {
+          
+        }
+        if ((0 < _LEN)) {
+          t256_4 <-
+          (VPBLEND_8u32 t256_2 t256_0
+          (W8.of_int
+          ((1 %% (2 ^ 1)) +
+          ((2 ^ 1) *
+          ((1 %% (2 ^ 1)) +
+          ((2 ^ 1) *
+          ((0 %% (2 ^ 1)) +
+          ((2 ^ 1) *
+          ((0 %% (2 ^ 1)) +
+          ((2 ^ 1) *
+          ((0 %% (2 ^ 1)) +
+          ((2 ^ 1) *
+          ((0 %% (2 ^ 1)) + ((2 ^ 1) * ((1 %% (2 ^ 1)) + ((2 ^ 1) * 1))))))))))))))
+          ));
+          (buf, dELTA, _LEN) <@ RW.MM.__a_ilen_write_upto32 (buf, offset, dELTA,
+          _LEN, t256_4);
+        } else {
+          
+        }
+        if ((0 < _LEN)) {
+          t <- (truncateu64 t128_0);
+          (buf, dELTA, _LEN) <@ RW.MM.__a_ilen_write_upto8 (buf, offset, dELTA,
+          _LEN, t);
+        } else {
+          
+        }
+        if ((0 < _LEN)) {
+          t256_4 <-
+          (VPBLEND_8u32 t256_1 t256_2
+          (W8.of_int
+          ((1 %% (2 ^ 1)) +
+          ((2 ^ 1) *
+          ((1 %% (2 ^ 1)) +
+          ((2 ^ 1) *
+          ((0 %% (2 ^ 1)) +
+          ((2 ^ 1) *
+          ((0 %% (2 ^ 1)) +
+          ((2 ^ 1) *
+          ((0 %% (2 ^ 1)) +
+          ((2 ^ 1) *
+          ((0 %% (2 ^ 1)) + ((2 ^ 1) * ((1 %% (2 ^ 1)) + ((2 ^ 1) * 1))))))))))))))
+          ));
+          (buf, dELTA, _LEN) <@ RW.MM.__a_ilen_write_upto32 (buf, offset, dELTA,
+          _LEN, t256_4);
+        } else {
+          
+        }
+      } else {
+        
+      }
+    } else {
+      
+    }
+    offset <- (offset + dELTA);
+    return (buf, offset);
+  }
+  proc __squeeze_avx2 (st:W256.t Array7.t, buf:W8.t A.t, _RATE8:int) : 
+  W256.t Array7.t * W8.t A.t = {
+    var _LEN:int;
+    var iTERS:int;
+    var lO:int;
+    var offset:int;
+    var i:int;
+    offset <- 0;
+    _LEN <- _ASIZE;
+    iTERS <- (_LEN %/ _RATE8);
+    lO <- (_LEN %% _RATE8);
+    i <- 0;
+    while ((i < iTERS)) {
+      st <@ M._keccakf1600_avx2 (st);
+      (buf, offset) <@ __dumpstate_avx2 (buf, offset, _RATE8, st);
+      i <- (i + 1);
+    }
+    if ((0 < lO)) {
+      st <@ M._keccakf1600_avx2 (st);
+      (buf, offset) <@ __dumpstate_avx2 (buf, offset, lO, st);
+    } else {
+      
+    }
+    return (st, buf);
+  }
+}.
+
+
+lemma addstate_avx2_ll: islossless MM.__addstate_avx2
+ by islossless.
+
+lemma absorb_avx2_ll: islossless MM.__absorb_avx2.
+proof.
+proc.
+seq 4: true => //=; last first.
+ if => //.
+ by call addratebit_avx2_ll.
+call addstate_avx2_ll.
+sp; if => //.
+ wp; while true (iTERS-i).
+ move=> z; wp.
+ call keccakf1600_avx2_ll.
+ call addstate_avx2_ll.
+ by auto => /#.
+wp; call keccakf1600_avx2_ll.
+wp; call addstate_avx2_ll.
+by auto => /#.
+qed.
+
+hoare absorb_avx2_h _l _buf _r8 _tb:
+ MM.__absorb_avx2
+ : aT = size _l %% _r8 /\ buf=_buf /\ _RATE8=_r8 /\ _TRAILB=_tb
+ /\ pabsorb_spec_avx2 _r8 _l st
+ ==> if _tb <> 0
+     then absorb_spec_avx2 _r8 _tb (_l ++ to_list _buf) res.`1
+     else pabsorb_spec_avx2 _r8 (_l ++ to_list _buf) res.`1
+          /\ res.`2 = (size _l + _ASIZE) %% _r8.
+proof.
+proc => /=.
+admitted.
+
+phoare absorb_avx2_ph _l _buf _r8 _tb:
+ [ MM.__absorb_avx2
+ : aT = size _l %% _r8 /\ buf=_buf /\ _RATE8=_r8 /\ _TRAILB=_tb
+ /\ pabsorb_spec_avx2 _r8 _l st
+ ==> if _tb <> 0
+     then absorb_spec_avx2 _r8 _tb (_l ++ to_list _buf) res.`1
+     else pabsorb_spec_avx2 _r8 (_l ++ to_list _buf) res.`1
+          /\ res.`2 = (size _l + _ASIZE) %% _r8
+ ] = 1%r.
+proof.
+by conseq absorb_avx2_ll (absorb_avx2_h _l _buf _r8 _tb).
+qed.
+
+(*
+   ONE-SHOT (FIXED-SIZE) MEMORY SQUEEZE
+   ====================================
+*)
+
+lemma dumpstate_avx2_ll: islossless MM.__dumpstate_avx2
+ by islossless.
+
+hoare dumpstate_avx2_h _buf _off _len _st:
+ MM.__dumpstate_avx2
+ : buf=_buf /\ offset=_off /\ _LEN=_len /\ st=_st
+ /\ 0 <= _len <= 200
+ ==> res.`1 = A.fill (fun i=>(stbytes (stavx2_to_st25 _st)).[i-_off]) _off _len _buf
+  /\ res.`2 = _off + _len.
+proof.
+proc => /=.
+admitted.
+
+phoare dumpstate_avx2_ph _buf _off _len _st:
+ [ MM.__dumpstate_avx2
+ : buf=_buf /\ offset=_off /\ _LEN=_len /\ st=_st
+ /\ 0 <= _len <= 200
+ ==> res.`1 = A.fill (fun i=>(stbytes (stavx2_to_st25 _st)).[i-_off]) _off _len _buf
+  /\ res.`2 = _off + _len
+ ] = 1%r.
+proof.
+have ?:= dumpstate_avx2_ll.
+have ?:= (dumpstate_avx2_h _buf _off _len _st).
+admit (* ????? anomaly: EcLib.EcCoreGoal.InvalidGoalShape ????
+by conseq dumpstate_avx2_ll (dumpstate_avx2_h _buf _off _len _st).
+*).
+qed.
+
+lemma squeeze_avx2_ll: islossless MM.__squeeze_avx2.
+proof.
+proc.
+seq 6: true => //.
+ while true (iTERS-i).
+  move=> z.
+  wp; call dumpstate_avx2_ll.
+  call keccakf1600_avx2_ll.
+  by auto => /#.
+ by auto => /#.
+if => //.
+call dumpstate_avx2_ll.
+call keccakf1600_avx2_ll.
+by auto.
+qed.
+
+hoare squeeze_avx2_h _buf _st _r8:
+ MM.__squeeze_avx2
+ : buf=_buf /\ st=_st /\ _RATE8=_r8
+ /\ 0 < _r8 <= 200
+ ==> res.`1 = stavx2_from_st25 (st_i (stavx2_to_st25 _st) ((_ASIZE-1) %/ _r8 + 1))
+     /\ to_list res.`2 = (SQUEEZE1600 _r8 _ASIZE (stavx2_to_st25 _st)).
+proof.
+proc.
+admitted.
+
+phoare squeeze_avx2_ph _buf _st _r8:
+ [ MM.__squeeze_avx2
+ : buf=_buf /\ st=_st /\ _RATE8=_r8
+ /\ 0 < _r8 <= 200
+ ==> res.`1 = stavx2_from_st25 (st_i (stavx2_to_st25 _st) ((_ASIZE-1) %/ _r8 + 1))
+     /\ to_list res.`2 = (SQUEEZE1600 _r8 _ASIZE (stavx2_to_st25 _st))
+ ] = 1%r.
+proof.
+by conseq squeeze_avx2_ll (squeeze_avx2_h _buf _st _r8).
+qed.
+
+end KeccakArrayAvx2.
