proof/amd64/avx2/Keccak1600_fixedsizes_avx2x4.ec
@@ -1,0 +1,869 @@
+(******************************************************************************
+   Keccak1600_imem_avx2.ec:
+
+   Correctness proof for the Keccak (fixed-sized) memory absorb/squeeze
+  4-way AVX2 implementation
+
+
+
+******************************************************************************)
+
+require import AllCore List Int IntDiv.
+
+from Jasmin require import JModel_x86.
+
+from JazzEC require import Keccak1600_Jazz.
+
+from JazzEC require import WArray200 WArray800.
+from JazzEC require import Array25.
+
+from CryptoSpecs require import JWordList.
+from CryptoSpecs require import FIPS202_Keccakf1600 Keccakf1600_Spec.
+from CryptoSpecs require import FIPS202_SHA3_Spec Keccak1600_Spec.
+
+
+require export Keccak1600_avx2x4 Keccakf1600_avx2x4.
+require import Keccak1600_subreadwrite.
+
+(*
+   INCREMENTAL (FIXED-SIZE) MEMORY ABSORB
+   ===================================
+*)
+
+lemma addstate_m_bcast_avx2x4_ll: islossless M.__addstate_m_bcast_avx2x4.
+proof.
+proc.
+seq 5: true => //.
+ while true (32 * (aT %/ 8 + _LEN %/ 8)-at).
+  by move=> z; auto => /#.
+ sp; if => //.
+  by wp; call m_ilen_read_bcast_upto8_at_ll; auto => /#.
+ by auto => /#.
+sp; if => //.
+by wp; call m_ilen_read_bcast_upto8_at_ll; auto => /#.
+qed.
+
+lemma addstate_m_avx2x4_ll: islossless M.__addstate_m_avx2x4.
+proof.
+proc.
+seq 5: true => //.
+ while true (4 * (aT %/ 8) + 4 * (_LEN %/ 8)-at).
+  by move=> z; auto => /#.
+ sp; if => //.
+  wp; call m_ilen_read_upto8_at_ll.
+  wp; call m_ilen_read_upto8_at_ll.
+  wp; call m_ilen_read_upto8_at_ll.
+  wp; call m_ilen_read_upto8_at_ll.
+  by auto => /#.
+ by auto => /#.
+sp; if => //.
+wp; call m_ilen_read_upto8_at_ll.
+wp; call m_ilen_read_upto8_at_ll.
+wp; call m_ilen_read_upto8_at_ll.
+wp; call m_ilen_read_upto8_at_ll.
+by auto => /#.
+qed.
+
+lemma absorb_m_bcast_avx2x4_ll: islossless M.__addstate_m_bcast_avx2x4.
+proof.
+proc.
+seq 7: true => //.
+ wp; while true (32 * (aT %/ 8 + _LEN %/ 8)-at).
+  by move => z; auto => /#.
+ sp; if => //.
+  by wp; call m_ilen_read_bcast_upto8_at_ll; auto => /#.
+ by auto => /#.
+if => //.
+by wp; call m_ilen_read_bcast_upto8_at_ll; auto => /#.
+qed.
+
+lemma absorb_m_avx2x4_ll: islossless M.__addstate_m_avx2x4.
+proof.
+proc.
+seq 7: true => //.
+ wp; while true (4 * (aT %/ 8) + 4 * (_LEN %/ 8)-at).
+  by move => z; auto => /#.
+ sp; if => //.
+  wp; call m_ilen_read_upto8_at_ll.
+  wp; call m_ilen_read_upto8_at_ll.
+  wp; call m_ilen_read_upto8_at_ll.
+  wp; call m_ilen_read_upto8_at_ll.
+  by auto => /#.
+ by auto => /#.
+if => //.
+wp; call m_ilen_read_upto8_at_ll.
+wp; call m_ilen_read_upto8_at_ll.
+wp; call m_ilen_read_upto8_at_ll.
+wp; call m_ilen_read_upto8_at_ll.
+by auto => /#.
+qed.
+
+(*
+   ONE-SHOT (FIXED-SIZE) MEMORY SQUEEZE
+   ====================================
+*)
+
+lemma dumpstate_m_avx2x4_ll: islossless M.__dumpstate_m_avx2x4.
+proof.
+proc.
+seq 7: true => //.
+ wp; while true (8 * (_LEN %/ 8)-i).
+  by move=> z; auto => /#.
+ while true (32 * (_LEN %/ 32)-i).
+  by move=> z; inline*; auto => /#.
+ by auto => /#.
+if => //.
+wp; call m_ilen_write_upto8_ll.
+wp; call m_ilen_write_upto8_ll.
+wp; call m_ilen_write_upto8_ll.
+wp; call m_ilen_write_upto8_ll.
+by auto => /#.
+qed.
+
+lemma squeeze_m_avx2x4_ll: islossless M.__squeeze_m_avx2x4.
+proof.
+proc.
+seq 3: true => //.
+ sp; if => //.
+ while true (iTERS-i).
+  move=> z.
+  wp; call dumpstate_m_avx2x4_ll.
+  wp; call keccakf1600_avx2x4_ll.
+  by auto => /#. 
+ by auto => /#.
+if => //.
+call  dumpstate_m_avx2x4_ll.
+by call keccakf1600_avx2x4_ll; auto => /#.
+qed.
+
+
+
+
+
+
+abstract theory KeccakArrayAvx2x4.
+
+op _ASIZE: int.
+
+axiom _ASIZE_ge0: 0 <= _ASIZE.
+axiom _ASIZE_u64: _ASIZE < W64.modulus.
+
+clone import PolyArray as A
+ with op size <- _ASIZE
+      proof ge0_size by exact _ASIZE_ge0.
+
+clone import WArray as WA
+ with op size <- _ASIZE.
+
+clone import ReadWriteArray as RW
+ with op _ASIZE <- _ASIZE,
+      theory A <- A,
+      theory WA <- WA
+      proof _ASIZE_ge0 by exact _ASIZE_ge0
+      proof _ASIZE_u64 by exact _ASIZE_u64.
+
+module MM = {
+  proc __addstate_bcast_avx2x4 (st:W256.t Array25.t, aT:int,
+                                buf:W8.t A.t, offset:int, _LEN:int,
+                                _TRAILB:int) : W256.t Array25.t * int * int = {
+    var dELTA:int;
+    var aT8:int;
+    var w:W256.t;
+    var at:int;
+    dELTA <- 0;
+    aT8 <- aT;
+    aT <- (8 * (aT %/ 8));
+    if (((aT8 %% 8) <> 0)) {
+      (dELTA, _LEN, _TRAILB, aT8, w) <@ RW.MM.__a_ilen_read_bcast_upto8_at (
+      buf, offset, dELTA, _LEN, _TRAILB, aT, aT8);
+      w <- (w `^` st.[(aT %/ 8)]);
+      st.[(aT %/ 8)] <- w;
+      aT <- aT8;
+    } else {
+      
+    }
+    offset <- (offset + dELTA);
+    at <- (32 * (aT %/ 8));
+    while ((at < (32 * ((aT %/ 8) + (_LEN %/ 8))))) {
+      w <-
+      (VPBROADCAST_4u64
+      (get64_direct (WA.init8 (fun i => buf.[i])) offset));
+      offset <- (offset + 8);
+      w <- (w `^` (get256_direct (WArray800.init256 (fun i => st.[i])) at));
+      st <-
+      (Array25.init
+      (WArray800.get256
+      (WArray800.set256_direct (WArray800.init256 (fun i => st.[i])) at w)));
+      at <- (at + 32);
+    }
+    aT <- (aT + (8 * (_LEN %/ 8)));
+    _LEN <- (_LEN %% 8);
+    if (((0 < _LEN) \/ ((_TRAILB %% 256) <> 0))) {
+      (dELTA, _LEN, _TRAILB, aT, w) <@ RW.MM.__a_ilen_read_bcast_upto8_at (
+      buf, offset, 0, _LEN, _TRAILB, aT, aT);
+      w <- (w `^` (get256_direct (WArray800.init256 (fun i => st.[i])) at));
+      st <-
+      (Array25.init
+      (WArray800.get256
+      (WArray800.set256_direct (WArray800.init256 (fun i => st.[i])) at w)));
+      offset <- (offset + dELTA);
+    } else {
+      
+    }
+    return (st, aT, offset);
+  }
+  proc __absorb_bcast_avx2x4 (st:W256.t Array25.t, aT:int,
+                              buf:W8.t A.t, _TRAILB:int, _RATE8:int) : 
+  W256.t Array25.t * int = {
+    var _LEN:int;
+    var iTERS:int;
+    var offset:int;
+    var i:int;
+    var  _0:int;
+    var  _1:int;
+    var  _2:int;
+    offset <- 0;
+    _LEN <- _ASIZE;
+    if ((_RATE8 <= (aT + _LEN))) {
+      (st,  _0, offset) <@ __addstate_bcast_avx2x4 (st, aT, buf, offset,
+      (_RATE8 - aT), 0);
+      _LEN <- (_LEN - (_RATE8 - aT));
+      aT <- 0;
+      st <@ M._keccakf1600_avx2x4 (st);
+      iTERS <- (_LEN %/ _RATE8);
+      i <- 0;
+      while ((i < iTERS)) {
+        (st,  _1, offset) <@ __addstate_bcast_avx2x4 (st, 0, buf, offset,
+        _RATE8, 0);
+        st <@ M._keccakf1600_avx2x4 (st);
+        i <- (i + 1);
+      }
+      _LEN <- (_LEN %% _RATE8);
+    } else {
+      
+    }
+    (st, aT,  _2) <@ __addstate_bcast_avx2x4 (st, aT, buf, offset, _LEN,
+    _TRAILB);
+    if ((_TRAILB <> 0)) {
+      st <@ M.__addratebit_avx2x4 (st, _RATE8);
+    } else {
+      
+    }
+    return (st, aT);
+  }
+  proc __addstate_avx2x4 (st:W256.t Array25.t, aT:int, buf0:W8.t A.t,
+                          buf1:W8.t A.t, buf2:W8.t A.t,
+                          buf3:W8.t A.t, offset:int, _LEN:int,
+                          _TRAILB:int) : W256.t Array25.t * int * int = {
+    var dELTA:int;
+    var aT8:int;
+    var t0:W64.t;
+    var t1:W64.t;
+    var t2:W64.t;
+    var t3:W64.t;
+    var at:int;
+    var  _0:int;
+    var  _1:int;
+    var  _2:int;
+    var  _3:int;
+    var  _4:int;
+    var  _5:int;
+    var  _6:int;
+    var  _7:int;
+    var  _8:int;
+    var  _9:int;
+    var  _10:int;
+    var  _11:int;
+    var  _12:int;
+    var  _13:int;
+    var  _14:int;
+    var  _15:int;
+    var  _16:int;
+    var  _17:int;
+    var  _18:int;
+    var  _19:int;
+    var  _20:int;
+    var  _21:int;
+    var  _22:int;
+    var  _23:int;
+    dELTA <- 0;
+    aT8 <- aT;
+    aT <- (8 * (aT %/ 8));
+    if (((aT8 %% 8) <> 0)) {
+      ( _0,  _1,  _2,  _3, t0) <@ RW.MM.__a_ilen_read_upto8_at (buf0, offset,
+      dELTA, _LEN, _TRAILB, aT, aT8);
+      st <-
+      (Array25.init
+      (WArray800.get256
+      (WArray800.set64 (WArray800.init256 (fun i => st.[i]))
+      ((4 * (aT %/ 8)) + 0)
+      ((get64 (WArray800.init256 (fun i => st.[i])) ((4 * (aT %/ 8)) + 0)) `^`
+      t0))));
+      ( _4,  _5,  _6,  _7, t1) <@ RW.MM.__a_ilen_read_upto8_at (buf1, offset,
+      dELTA, _LEN, _TRAILB, aT, aT8);
+      st <-
+      (Array25.init
+      (WArray800.get256
+      (WArray800.set64 (WArray800.init256 (fun i => st.[i]))
+      ((4 * (aT %/ 8)) + 1)
+      ((get64 (WArray800.init256 (fun i => st.[i])) ((4 * (aT %/ 8)) + 1)) `^`
+      t1))));
+      ( _8,  _9,  _10,  _11, t2) <@ RW.MM.__a_ilen_read_upto8_at (buf2, offset,
+      dELTA, _LEN, _TRAILB, aT, aT8);
+      st <-
+      (Array25.init
+      (WArray800.get256
+      (WArray800.set64 (WArray800.init256 (fun i => st.[i]))
+      ((4 * (aT %/ 8)) + 2)
+      ((get64 (WArray800.init256 (fun i => st.[i])) ((4 * (aT %/ 8)) + 2)) `^`
+      t2))));
+      (dELTA, _LEN, _TRAILB, aT8, t3) <@ RW.MM.__a_ilen_read_upto8_at (buf3,
+      offset, dELTA, _LEN, _TRAILB, aT, aT8);
+      st <-
+      (Array25.init
+      (WArray800.get256
+      (WArray800.set64 (WArray800.init256 (fun i => st.[i]))
+      ((4 * (aT %/ 8)) + 3)
+      ((get64 (WArray800.init256 (fun i => st.[i])) ((4 * (aT %/ 8)) + 3)) `^`
+      t3))));
+      aT <- aT8;
+    } else {
+      
+    }
+    offset <- (offset + dELTA);
+    at <- (4 * (aT %/ 8));
+    while ((at < ((4 * (aT %/ 8)) + (4 * (_LEN %/ 8))))) {
+      t0 <- (get64_direct (WA.init8 (fun i => buf0.[i])) offset);
+      st <-
+      (Array25.init
+      (WArray800.get256
+      (WArray800.set64 (WArray800.init256 (fun i => st.[i])) (at + 0)
+      ((get64 (WArray800.init256 (fun i => st.[i])) (at + 0)) `^` t0))));
+      t1 <- (get64_direct (WA.init8 (fun i => buf1.[i])) offset);
+      st <-
+      (Array25.init
+      (WArray800.get256
+      (WArray800.set64 (WArray800.init256 (fun i => st.[i])) (at + 1)
+      ((get64 (WArray800.init256 (fun i => st.[i])) (at + 1)) `^` t1))));
+      t2 <- (get64_direct (WA.init8 (fun i => buf2.[i])) offset);
+      st <-
+      (Array25.init
+      (WArray800.get256
+      (WArray800.set64 (WArray800.init256 (fun i => st.[i])) (at + 2)
+      ((get64 (WArray800.init256 (fun i => st.[i])) (at + 2)) `^` t2))));
+      t3 <- (get64_direct (WA.init8 (fun i => buf3.[i])) offset);
+      offset <- (offset + 8);
+      st <-
+      (Array25.init
+      (WArray800.get256
+      (WArray800.set64 (WArray800.init256 (fun i => st.[i])) (at + 3)
+      ((get64 (WArray800.init256 (fun i => st.[i])) (at + 3)) `^` t3))));
+      at <- (at + 4);
+    }
+    aT <- (aT + (8 * (_LEN %/ 8)));
+    _LEN <- (_LEN %% 8);
+    if (((0 < _LEN) \/ ((_TRAILB %% 256) <> 0))) {
+      ( _12,  _13,  _14,  _15, t0) <@ RW.MM.__a_ilen_read_upto8_at (buf0, offset,
+      0, _LEN, _TRAILB, aT, aT);
+      st <-
+      (Array25.init
+      (WArray800.get256
+      (WArray800.set64 (WArray800.init256 (fun i => st.[i])) (at + 0)
+      ((get64 (WArray800.init256 (fun i => st.[i])) (at + 0)) `^` t0))));
+      ( _16,  _17,  _18,  _19, t1) <@ RW.MM.__a_ilen_read_upto8_at (buf1, offset,
+      0, _LEN, _TRAILB, aT, aT);
+      st <-
+      (Array25.init
+      (WArray800.get256
+      (WArray800.set64 (WArray800.init256 (fun i => st.[i])) (at + 1)
+      ((get64 (WArray800.init256 (fun i => st.[i])) (at + 1)) `^` t1))));
+      ( _20,  _21,  _22,  _23, t2) <@ RW.MM.__a_ilen_read_upto8_at (buf2, offset,
+      0, _LEN, _TRAILB, aT, aT);
+      st <-
+      (Array25.init
+      (WArray800.get256
+      (WArray800.set64 (WArray800.init256 (fun i => st.[i])) (at + 2)
+      ((get64 (WArray800.init256 (fun i => st.[i])) (at + 2)) `^` t2))));
+      (dELTA, _LEN, _TRAILB, aT, t3) <@ RW.MM.__a_ilen_read_upto8_at (buf3, 
+      offset, 0, _LEN, _TRAILB, aT, aT);
+      st <-
+      (Array25.init
+      (WArray800.get256
+      (WArray800.set64 (WArray800.init256 (fun i => st.[i])) (at + 3)
+      ((get64 (WArray800.init256 (fun i => st.[i])) (at + 3)) `^` t3))));
+      offset <- (offset + dELTA);
+    } else {
+      
+    }
+    return (st, aT, offset);
+  }
+  proc __absorb_avx2x4 (st:W256.t Array25.t, aT:int, buf0:W8.t A.t,
+                        buf1:W8.t A.t, buf2:W8.t A.t,
+                        buf3:W8.t A.t, _TRAILB:int, _RATE8:int) : 
+  W256.t Array25.t * int = {
+    var _LEN:int;
+    var iTERS:int;
+    var offset:int;
+    var i:int;
+    var  _0:int;
+    var  _1:int;
+    var  _2:int;
+    offset <- 0;
+    _LEN <- _ASIZE;
+    if ((_RATE8 <= (aT + _LEN))) {
+      (st,  _0, offset) <@ __addstate_avx2x4 (st, aT, buf0, buf1, buf2, 
+      buf3, offset, (_RATE8 - aT), 0);
+      _LEN <- (_LEN - (_RATE8 - aT));
+      aT <- 0;
+      st <@ M._keccakf1600_avx2x4 (st);
+      iTERS <- (_LEN %/ _RATE8);
+      i <- 0;
+      while ((i < iTERS)) {
+        (st,  _1, offset) <@ __addstate_avx2x4 (st, 0, buf0, buf1, buf2,
+        buf3, offset, _RATE8, 0);
+        st <@ M._keccakf1600_avx2x4 (st);
+        i <- (i + 1);
+      }
+      _LEN <- (_LEN %% _RATE8);
+    } else {
+      
+    }
+    (st, aT,  _2) <@ __addstate_avx2x4 (st, aT, buf0, buf1, buf2, buf3,
+    offset, _LEN, _TRAILB);
+    if ((_TRAILB <> 0)) {
+      st <@ M.__addratebit_avx2x4 (st, _RATE8);
+    } else {
+      
+    }
+    return (st, aT);
+  }
+  proc __dumpstate_avx2x4 (buf0:W8.t A.t, buf1:W8.t A.t,
+                           buf2:W8.t A.t, buf3:W8.t A.t,
+                           offset:int, _LEN:int, st:W256.t Array25.t) : 
+  W8.t A.t * W8.t A.t * W8.t A.t * W8.t A.t * int = {
+    var x0:W256.t;
+    var x1:W256.t;
+    var x2:W256.t;
+    var x3:W256.t;
+    var t0:W64.t;
+    var t1:W64.t;
+    var t2:W64.t;
+    var t3:W64.t;
+    var i:int;
+    var  _0:int;
+    var  _1:int;
+    var  _2:int;
+    var  _3:int;
+    var  _4:int;
+    var  _5:int;
+    var  _6:int;
+    var  _7:int;
+    i <- 0;
+    while ((i < (32 * (_LEN %/ 32)))) {
+      x0 <-
+      (get256_direct (WArray800.init256 (fun i_0 => st.[i_0]))
+      ((4 * i) + (0 * 32)));
+      x1 <-
+      (get256_direct (WArray800.init256 (fun i_0 => st.[i_0]))
+      ((4 * i) + (1 * 32)));
+      x2 <-
+      (get256_direct (WArray800.init256 (fun i_0 => st.[i_0]))
+      ((4 * i) + (2 * 32)));
+      x3 <-
+      (get256_direct (WArray800.init256 (fun i_0 => st.[i_0]))
+      ((4 * i) + (3 * 32)));
+      i <- (i + 32);
+      (x0, x1, x2, x3) <@ M.__4u64x4_u256x4 (x0, x1, x2, x3);
+      buf0 <-
+      (A.init
+      (WA.get8
+      (WA.set256_direct (WA.init8 (fun i_0 => buf0.[i_0]))
+      offset x0)));
+      buf1 <-
+      (A.init
+      (WA.get8
+      (WA.set256_direct (WA.init8 (fun i_0 => buf1.[i_0]))
+      offset x1)));
+      buf2 <-
+      (A.init
+      (WA.get8
+      (WA.set256_direct (WA.init8 (fun i_0 => buf2.[i_0]))
+      offset x2)));
+      buf3 <-
+      (A.init
+      (WA.get8
+      (WA.set256_direct (WA.init8 (fun i_0 => buf3.[i_0]))
+      offset x3)));
+      offset <- (offset + 32);
+    }
+    while ((i < (8 * (_LEN %/ 8)))) {
+      t0 <-
+      (get64_direct (WArray800.init256 (fun i_0 => st.[i_0]))
+      ((4 * i) + (0 * 8)));
+      buf0 <-
+      (A.init
+      (WA.get8
+      (WA.set64_direct (WA.init8 (fun i_0 => buf0.[i_0]))
+      offset t0)));
+      t1 <-
+      (get64_direct (WArray800.init256 (fun i_0 => st.[i_0]))
+      ((4 * i) + (1 * 8)));
+      buf1 <-
+      (A.init
+      (WA.get8
+      (WA.set64_direct (WA.init8 (fun i_0 => buf1.[i_0]))
+      offset t1)));
+      t2 <-
+      (get64_direct (WArray800.init256 (fun i_0 => st.[i_0]))
+      ((4 * i) + (2 * 8)));
+      buf2 <-
+      (A.init
+      (WA.get8
+      (WA.set64_direct (WA.init8 (fun i_0 => buf2.[i_0]))
+      offset t2)));
+      t3 <-
+      (get64_direct (WArray800.init256 (fun i_0 => st.[i_0]))
+      ((4 * i) + (3 * 8)));
+      buf3 <-
+      (A.init
+      (WA.get8
+      (WA.set64_direct (WA.init8 (fun i_0 => buf3.[i_0]))
+      offset t3)));
+      i <- (i + 8);
+      offset <- (offset + 8);
+    }
+    if ((0 < (_LEN %% 8))) {
+      t0 <-
+      (get64_direct (WArray800.init256 (fun i_0 => st.[i_0]))
+      ((4 * i) + (0 * 8)));
+      (buf0,  _0,  _1) <@ RW.MM.__a_ilen_write_upto8 (buf0, offset, 0, (_LEN %% 8),
+      t0);
+      t1 <-
+      (get64_direct (WArray800.init256 (fun i_0 => st.[i_0]))
+      ((4 * i) + (1 * 8)));
+      (buf1,  _2,  _3) <@ RW.MM.__a_ilen_write_upto8 (buf1, offset, 0, (_LEN %% 8),
+      t1);
+      t2 <-
+      (get64_direct (WArray800.init256 (fun i_0 => st.[i_0]))
+      ((4 * i) + (2 * 8)));
+      (buf2,  _4,  _5) <@ RW.MM.__a_ilen_write_upto8 (buf2, offset, 0, (_LEN %% 8),
+      t2);
+      t3 <-
+      (get64_direct (WArray800.init256 (fun i_0 => st.[i_0]))
+      ((4 * i) + (3 * 8)));
+      (buf3,  _6,  _7) <@ RW.MM.__a_ilen_write_upto8 (buf3, offset, 0, (_LEN %% 8),
+      t3);
+      offset <- (offset + (_LEN %% 8));
+    } else {
+      
+    }
+    return (buf0, buf1, buf2, buf3, offset);
+  }
+  proc __squeeze_avx2x4 (st:W256.t Array25.t, buf0:W8.t A.t,
+                         buf1:W8.t A.t, buf2:W8.t A.t,
+                         buf3:W8.t A.t, _RATE8:int) : W256.t Array25.t *
+                                                             W8.t A.t *
+                                                             W8.t A.t *
+                                                             W8.t A.t *
+                                                             W8.t A.t = {
+    var _LEN:int;
+    var iTERS:int;
+    var lO:int;
+    var offset:int;
+    var i:int;
+    offset <- 0;
+    _LEN <- _ASIZE;
+    iTERS <- (_LEN %/ _RATE8);
+    lO <- (_LEN %% _RATE8);
+    if ((0 < iTERS)) {
+      i <- 0;
+      while ((i < iTERS)) {
+        st <@ M._keccakf1600_avx2x4 (st);
+        (buf0, buf1, buf2, buf3, offset) <@ __dumpstate_avx2x4 (buf0, 
+        buf1, buf2, buf3, offset, _RATE8, st);
+        i <- (i + 1);
+      }
+    } else {
+      
+    }
+    if ((0 < lO)) {
+      st <@ M._keccakf1600_avx2x4 (st);
+      (buf0, buf1, buf2, buf3, offset) <@ __dumpstate_avx2x4 (buf0, buf1,
+      buf2, buf3, offset, lO, st);
+    } else {
+      
+    }
+    return (st, buf0, buf1, buf2, buf3);
+  }
+}.
+
+
+(*
+   INCREMENTAL (FIXED-SIZE) MEMORY ABSORB
+   ===================================
+*)
+
+lemma addstate_bcast_avx2x4_ll: islossless MM.__addstate_bcast_avx2x4.
+proof.
+proc.
+seq 7: true => //.
+ while true (32 * (aT %/ 8 + _LEN %/ 8)-at).
+  by move=> z; auto => /#.
+ sp; if => //.
+  by wp; call a_ilen_read_bcast_upto8_at_ll; auto => /#.
+ by auto => /#.
+sp; if => //.
+by wp; call a_ilen_read_bcast_upto8_at_ll; auto => /#.
+qed.
+
+lemma addstate_avx2x4_ll: islossless MM.__addstate_avx2x4.
+proof.
+proc.
+seq 7: true => //.
+ while true (4 * (aT %/ 8) + 4 * (_LEN %/ 8)-at).
+  by move=> z; auto => /#.
+ sp; if => //.
+  wp; call a_ilen_read_upto8_at_ll.
+  wp; call a_ilen_read_upto8_at_ll.
+  wp; call a_ilen_read_upto8_at_ll.
+  wp; call a_ilen_read_upto8_at_ll.
+  by auto => /#.
+ by auto => /#.
+sp; if => //.
+wp; call a_ilen_read_upto8_at_ll.
+wp; call a_ilen_read_upto8_at_ll.
+wp; call a_ilen_read_upto8_at_ll.
+wp; call a_ilen_read_upto8_at_ll.
+by auto => /#.
+qed.
+
+lemma absorb_bcast_avx2x4_ll: islossless MM.__absorb_bcast_avx2x4.
+proof.
+proc.
+seq 4: true => //.
+ call addstate_bcast_avx2x4_ll.
+ sp; if => //.
+ wp; while true (iTERS-i).
+  move => z.
+  wp; call keccakf1600_avx2x4_ll.
+  wp; call addstate_bcast_avx2x4_ll.
+  by auto => /#.
+ wp; call keccakf1600_avx2x4_ll.
+ wp; call addstate_bcast_avx2x4_ll.
+ by auto => /#.
+if => //.
+by call addratebit_avx2x4_ll.
+qed.
+
+hoare absorb_bcast_avx2x4_h _l0 _l1 _l2 _l3 _st _buf _r8 _tb:
+ MM.__absorb_bcast_avx2x4
+ : st=_st /\ buf=_buf /\ _RATE8 = _r8 /\ _TRAILB=_tb
+ /\ aT = size _l0 %% _r8 /\ size _l1 = size _l0 /\ size _l2 = size _l0 /\ size _l3 = size _l0
+ /\ pabsorb_spec_avx2x4 _r8 _l0 _l1 _l2 _l3 _st
+ ==> if _tb <> 0
+     then absorb_spec_avx2x4 _r8 _tb
+            (_l0 ++ to_list _buf)
+            (_l1 ++ to_list _buf)
+            (_l2 ++ to_list _buf)
+            (_l3 ++ to_list _buf)
+            res.`1
+     else pabsorb_spec_avx2x4 _r8
+            (_l0 ++ to_list _buf)
+            (_l1 ++ to_list _buf)
+            (_l2 ++ to_list _buf)
+            (_l3 ++ to_list _buf)
+            res.`1
+           /\ res.`2 = (size _l0 + _ASIZE) %% _r8.
+proof.
+proc.
+admitted.
+
+phoare absorb_bcast_avx2x4_ph _l0 _l1 _l2 _l3 _st _buf _r8 _tb:
+ [ MM.__absorb_bcast_avx2x4
+ : st=_st /\ buf=_buf /\ _RATE8 = _r8 /\ _TRAILB=_tb
+ /\ aT = size _l0 %% _r8 /\ size _l1 = size _l0 /\ size _l2 = size _l0 /\ size _l3 = size _l0
+ /\ pabsorb_spec_avx2x4 _r8 _l0 _l1 _l2 _l3 _st
+ ==> if _tb <> 0
+     then absorb_spec_avx2x4 _r8 _tb
+            (_l0 ++ to_list _buf)
+            (_l1 ++ to_list _buf)
+            (_l2 ++ to_list _buf)
+            (_l3 ++ to_list _buf)
+            res.`1
+     else pabsorb_spec_avx2x4 _r8
+            (_l0 ++ to_list _buf)
+            (_l1 ++ to_list _buf)
+            (_l2 ++ to_list _buf)
+            (_l3 ++ to_list _buf)
+            res.`1
+           /\ res.`2 = (size _l0 + _ASIZE) %% _r8
+  ] = 1%r.
+proof.
+by conseq absorb_bcast_avx2x4_ll (absorb_bcast_avx2x4_h _l0 _l1 _l2 _l3 _st _buf _r8 _tb).
+qed.
+
+lemma absorb_avx2x4_ll: islossless MM.__absorb_avx2x4.
+proof.
+proc.
+seq 4: true => //.
+ call addstate_avx2x4_ll.
+ sp; if => //.
+ wp; while true (iTERS-i).
+  move => z.
+  wp; call keccakf1600_avx2x4_ll.
+  call addstate_avx2x4_ll.
+  by auto => /#.
+ wp; call keccakf1600_avx2x4_ll.
+ by wp; call addstate_avx2x4_ll; auto => /#.
+if => //.
+by call addratebit_avx2x4_ll.
+qed.
+
+hoare absorb_avx2x4_h _l0 _l1 _l2 _l3 _st _buf0 _buf1 _buf2 _buf3 _r8 _tb:
+ MM.__absorb_avx2x4
+ : st=_st /\ buf0=_buf0 /\ buf1=_buf1 /\ buf2=_buf2 /\ buf3=_buf3 /\
+ _RATE8 = _r8 /\ _TRAILB=_tb
+ /\ aT = size _l0 %% _r8 /\ size _l1 = size _l0 /\ size _l2 = size _l0 /\ size _l3 = size _l0
+ /\ pabsorb_spec_avx2x4 _r8 _l0 _l1 _l2 _l3 _st
+ ==> if _tb <> 0
+     then absorb_spec_avx2x4 _r8 _tb
+            (_l0 ++ to_list _buf0)
+            (_l1 ++ to_list _buf1)
+            (_l2 ++ to_list _buf2)
+            (_l3 ++ to_list _buf3)
+            res.`1
+     else pabsorb_spec_avx2x4 _r8
+            (_l0 ++ to_list _buf0)
+            (_l1 ++ to_list _buf1)
+            (_l2 ++ to_list _buf2)
+            (_l3 ++ to_list _buf3)
+            res.`1
+           /\ res.`2 = (size _l0 + _ASIZE) %% _r8.
+admitted.
+
+phoare absorb_avx2x4_ph _l0 _l1 _l2 _l3 _st _buf0 _buf1 _buf2 _buf3 _r8 _tb:
+ [ MM.__absorb_avx2x4
+ : st=_st /\ buf0=_buf0 /\ buf1=_buf1 /\ buf2=_buf2 /\ buf3=_buf3 /\
+ _RATE8 = _r8 /\ _TRAILB=_tb
+ /\ aT = size _l0 %% _r8 /\ size _l1 = size _l0 /\ size _l2 = size _l0 /\ size _l3 = size _l0
+ /\ pabsorb_spec_avx2x4 _r8 _l0 _l1 _l2 _l3 _st
+ ==> if _tb <> 0
+     then absorb_spec_avx2x4 _r8 _tb
+            (_l0 ++ to_list _buf0)
+            (_l1 ++ to_list _buf1)
+            (_l2 ++ to_list _buf2)
+            (_l3 ++ to_list _buf3)
+            res.`1
+     else pabsorb_spec_avx2x4 _r8
+            (_l0 ++ to_list _buf0)
+            (_l1 ++ to_list _buf1)
+            (_l2 ++ to_list _buf2)
+            (_l3 ++ to_list _buf3)
+            res.`1
+           /\ res.`2 = (size _l0 + _ASIZE) %% _r8
+  ] = 1%r.
+proof.
+by conseq absorb_avx2x4_ll (absorb_avx2x4_h _l0 _l1 _l2 _l3 _st _buf0 _buf1 _buf2 _buf3 _r8 _tb).
+qed.
+
+(*
+   ONE-SHOT (FIXED-SIZE) MEMORY SQUEEZE
+   ====================================
+*)
+
+lemma dumpstate_avx2x4_ll: islossless MM.__dumpstate_avx2x4.
+proof.
+proc.
+seq 3: true => //.
+ while true (8 * (_LEN %/ 8)-i).
+  by move=> z; auto => /#.
+ while true (32 * (_LEN %/ 32)-i).
+  by move=> z; inline*; auto => /#.
+ by auto => /#.
+if => //.
+wp; call a_ilen_write_upto8_ll.
+wp; call a_ilen_write_upto8_ll.
+wp; call a_ilen_write_upto8_ll.
+wp; call a_ilen_write_upto8_ll.
+by auto => /#.
+qed.
+
+hoare dumpstate_avx2x4_h _buf0 _buf1 _buf2 _buf3 _off _len _st:
+ MM.__dumpstate_avx2x4
+ : buf0=_buf0 /\ buf1=_buf1 /\ buf2=_buf2 /\ buf3=_buf3 /\ offset=_off /\ _LEN=_len /\ st=_st
+ /\ 0 <= _len <= 200
+ /\ _off + _len <= _ASIZE
+ ==> res.`1 = A.fill (fun i=> (stbytes (st4x_get _st 0)).[i-_off]) _off _len _buf0
+  /\ res.`2 = A.fill (fun i=> (stbytes (st4x_get _st 1)).[i-_off]) _off _len _buf1
+  /\ res.`3 = A.fill (fun i=> (stbytes (st4x_get _st 2)).[i-_off]) _off _len _buf2
+  /\ res.`4 = A.fill (fun i=> (stbytes (st4x_get _st 3)).[i-_off]) _off _len _buf3
+  /\ res.`5 = _off + _len.
+admitted.
+
+phoare dumpstate_avx2x4_ph _buf0 _buf1 _buf2 _buf3 _off _len _st:
+ [ MM.__dumpstate_avx2x4
+ : buf0=_buf0 /\ buf1=_buf1 /\ buf2=_buf2 /\ buf3=_buf3 /\ offset=_off /\ _LEN=_len /\ st=_st
+ /\ 0 <= _len <= 200
+ /\ _off + _len <= _ASIZE
+ ==> res.`1 = A.fill (fun i=> (stbytes (st4x_get _st 0)).[i-_off]) _off _len _buf0
+  /\ res.`2 = A.fill (fun i=> (stbytes (st4x_get _st 1)).[i-_off]) _off _len _buf1
+  /\ res.`3 = A.fill (fun i=> (stbytes (st4x_get _st 2)).[i-_off]) _off _len _buf2
+  /\ res.`4 = A.fill (fun i=> (stbytes (st4x_get _st 3)).[i-_off]) _off _len _buf3
+  /\ res.`5 = _off + _len
+  ] = 1%r.
+proof.
+admit (* ??? anomaly: EcLib.EcCoreGoal.InvalidGoalShape 
+by conseq dumpstate_avx2x4_ll (dumpstate_avx2x4_h _buf0 _buf1 _buf2 _buf3 _off _len _st).
+*).
+qed.
+
+lemma squeeze_avx2x4_ll: islossless MM.__squeeze_avx2x4.
+proof.
+proc.
+seq 5: true => //.
+ sp; if => //.
+ while true (iTERS-i).
+  move=> z.
+  wp; call dumpstate_avx2x4_ll.
+  wp; call keccakf1600_avx2x4_ll.
+  by auto => /#. 
+ by auto => /#.
+if => //.
+call  dumpstate_avx2x4_ll.
+by call keccakf1600_avx2x4_ll; auto => /#.
+qed.
+
+hoare squeeze_avx2x4_h _buf0 _buf1 _buf2 _buf3 _st _r8:
+ MM.__squeeze_avx2x4
+ : buf0=_buf0 /\ buf1=_buf1 /\ buf2=_buf2 /\ buf3=_buf3
+ /\ st=_st /\ _RATE8=_r8
+ /\ 0 < _r8 <= 200
+ ==>
+    res.`1 = iter ((_ASIZE - 1) %/ _r8 + 1) keccak_f1600_x4 _st
+ /\ to_list res.`2 = SQUEEZE1600 _r8 _ASIZE (st4x_get _st 0)
+ /\ to_list res.`3 = SQUEEZE1600 _r8 _ASIZE (st4x_get _st 1)
+ /\ to_list res.`4 = SQUEEZE1600 _r8 _ASIZE (st4x_get _st 2)
+ /\ to_list res.`5 = SQUEEZE1600 _r8 _ASIZE (st4x_get _st 3).
+admitted.
+
+phoare squeeze_avx2x4_ph _buf0 _buf1 _buf2 _buf3 _st _r8:
+ [ MM.__squeeze_avx2x4
+ : buf0=_buf0 /\ buf1=_buf1 /\ buf2=_buf2 /\ buf3=_buf3
+ /\ st=_st /\ _RATE8=_r8
+ /\ 0 < _r8 <= 200
+ ==>
+    res.`1 = iter ((_ASIZE - 1) %/ _r8 + 1) keccak_f1600_x4 _st
+ /\ to_list res.`2 = SQUEEZE1600 _r8 _ASIZE (st4x_get _st 0)
+ /\ to_list res.`3 = SQUEEZE1600 _r8 _ASIZE (st4x_get _st 1)
+ /\ to_list res.`4 = SQUEEZE1600 _r8 _ASIZE (st4x_get _st 2)
+ /\ to_list res.`5 = SQUEEZE1600 _r8 _ASIZE (st4x_get _st 3)
+ ] = 1%r.
+proof.
+admit (* ??? anomaly: EcLib.EcCoreGoal.InvalidGoalShape
+by conseq squeeze_avx2x4_ll (squeeze_avx2x4_h _buf0 _buf1 _buf2 _buf3 _st _r8).
+*).
+qed.
+
+end KeccakArrayAvx2x4.
+
+
