proof/amd64/common/Keccak1600_subreadwrite.ec
@@ -1,0 +1,527 @@
+require import AllCore IntDiv CoreMap List Distr.
+
+from Jasmin require import JModel_x86.
+from JazzEC require import Keccak1600_Jazz.
+
+import SLH64.
+
+
+lemma SHLQ_ll: islossless M.__SHLQ
+by islossless.
+
+lemma SHLDQ_ll: islossless M.__SHLDQ
+by islossless.
+
+lemma SHLQ_256_ll: islossless M.__SHLQ_256
+by islossless.
+
+lemma m_ilen_read_upto8_at_ll: islossless M.__m_ilen_read_upto8_at
+by islossless.
+
+lemma m_ilen_read_upto16_at_ll: islossless M.__m_ilen_read_upto16_at
+by islossless.
+
+lemma m_ilen_read_upto32_at_ll: islossless M.__m_ilen_read_upto32_at
+by islossless.
+
+lemma m_ilen_read_bcast_upto8_at_ll: islossless M.__m_ilen_read_bcast_upto8_at
+by islossless.
+
+lemma m_ilen_write_upto8_ll: islossless M.__m_ilen_write_upto8
+by islossless.
+
+lemma m_ilen_write_upto16_ll: islossless M.__m_ilen_write_upto8
+by islossless.
+
+lemma m_ilen_write_upto32_ll: islossless M.__m_ilen_write_upto32
+by islossless.
+
+lemma m_rlen_read_upto8_ll: islossless M.__m_rlen_read_upto8
+by islossless.
+
+lemma m_rlen_write_upto8_ll: islossless M.__m_rlen_write_upto8
+by islossless.
+
+
+
+abstract theory ReadWriteArray.
+
+op _ASIZE: int.
+
+axiom _ASIZE_ge0: 0 <= _ASIZE.
+axiom _ASIZE_u64: _ASIZE < W64.modulus.
+
+clone import PolyArray as A
+ with op size <- _ASIZE
+      proof ge0_size by exact _ASIZE_ge0.
+
+clone import WArray as WA
+ with op size <- _ASIZE.
+
+module MM = {
+  proc __a_ilen_read_upto8_at (buf:W8.t A.t, offset:int, dELTA:int,
+                               lEN:int, tRAIL:int, cUR:int, aT:int) : 
+  int * int * int * int * W64.t = {
+    var w:W64.t;
+    var aT8:int;
+    var t16:W64.t;
+    var t8:W64.t;
+    if ((((aT < cUR) \/ ((cUR + 8) <= aT)) \/ ((lEN = 0) /\ (tRAIL = 0)))) {
+      w <- (W64.of_int 0);
+    } else {
+      aT8 <- (aT - cUR);
+      if ((8 <= lEN)) {
+        w <-
+        (get64_direct (WA.init8 (fun i => buf.[i]))
+        (W64.to_uint ((W64.of_int offset) + (W64.of_int dELTA))));
+        w <@ M.__SHLQ (w, aT8);
+        dELTA <- (dELTA + (8 - aT8));
+        lEN <- (lEN - (8 - aT8));
+        aT8 <- 8;
+      } else {
+        if ((4 <= lEN)) {
+          w <-
+          (zeroextu64
+          (get32_direct (WA.init8 (fun i => buf.[i]))
+          (W64.to_uint ((W64.of_int offset) + (W64.of_int dELTA)))));
+          w <@ M.__SHLQ (w, aT8);
+          dELTA <- (dELTA + ((8 <= (4 + aT8)) ? (8 - aT8) : 4));
+          lEN <- (lEN - ((8 <= (4 + aT8)) ? (8 - aT8) : 4));
+          aT8 <- ((8 <= (4 + aT8)) ? 8 : (4 + aT8));
+        } else {
+          w <- (W64.of_int 0);
+        }
+        if (((aT8 < 8) /\ (2 <= lEN))) {
+          t16 <-
+          (zeroextu64
+          (get16_direct (WA.init8 (fun i => buf.[i]))
+          (W64.to_uint ((W64.of_int offset) + (W64.of_int dELTA)))));
+          dELTA <- (dELTA + ((8 <= (2 + aT8)) ? (8 - aT8) : 2));
+          lEN <- (lEN - ((8 <= (2 + aT8)) ? (8 - aT8) : 2));
+          t16 <@ M.__SHLQ (t16, aT8);
+          w <- (w `|` t16);
+          aT8 <- ((8 <= (2 + aT8)) ? 8 : (2 + aT8));
+        } else {
+          
+        }
+        if ((aT8 < 8)) {
+          if ((1 <= lEN)) {
+            t8 <-
+            (zeroextu64
+            (get8_direct (WA.init8 (fun i => buf.[i]))
+            (W64.to_uint ((W64.of_int offset) + (W64.of_int dELTA)))));
+            t8 <- (t8 `|` (W64.of_int (256 * (tRAIL %% 256))));
+            dELTA <- (dELTA + 1);
+            lEN <- (lEN - 1);
+            t8 <@ M.__SHLQ (t8, aT8);
+            w <- (w `|` t8);
+            aT8 <- (aT8 + 1);
+            if (((aT8 < 8) /\ ((tRAIL %% 256) <> 0))) {
+              aT8 <- (aT8 + 1);
+              tRAIL <- 0;
+            } else {
+              
+            }
+          } else {
+            if (((tRAIL %% 256) <> 0)) {
+              t8 <- (W64.of_int (tRAIL %% 256));
+              t8 <@ M.__SHLQ (t8, aT8);
+              w <- (w `|` t8);
+              tRAIL <- 0;
+              aT8 <- (aT8 + 1);
+            } else {
+              
+            }
+          }
+        } else {
+          
+        }
+      }
+      aT <- (cUR + aT8);
+    }
+    return (dELTA, lEN, tRAIL, aT, w);
+  }
+  proc __a_ilen_read_upto16_at (buf:W8.t A.t, offset:int, dELTA:int,
+                                lEN:int, tRAIL:int, cUR:int, aT:int) : 
+  int * int * int * int * W128.t = {
+    var w:W128.t;
+    var aT16:int;
+    var t64_0:W64.t;
+    var t64_1:W64.t;
+    if ((((aT < cUR) \/ ((cUR + 16) <= aT)) \/ ((lEN = 0) /\ (tRAIL = 0)))) {
+      w <- (set0_128);
+    } else {
+      aT16 <- (aT - cUR);
+      if ((16 <= lEN)) {
+        w <-
+        (get128_direct (WA.init8 (fun i => buf.[i]))
+        (W64.to_uint ((W64.of_int offset) + (W64.of_int dELTA))));
+        w <@ M.__SHLDQ (w, aT16);
+        dELTA <- (dELTA + (16 - aT16));
+        lEN <- (lEN - (16 - aT16));
+        aT16 <- 16;
+      } else {
+        if ((8 <= aT16)) {
+          w <- (set0_128);
+          (dELTA, lEN, tRAIL, aT16, t64_1) <@ __a_ilen_read_upto8_at (
+          buf, offset, dELTA, lEN, tRAIL, 8, aT16);
+          w <- (VPINSR_2u64 w t64_1 (W8.of_int 1));
+        } else {
+          (dELTA, lEN, tRAIL, aT16, t64_0) <@ __a_ilen_read_upto8_at (
+          buf, offset, dELTA, lEN, tRAIL, 0, aT16);
+          w <- (zeroextu128 t64_0);
+          (dELTA, lEN, tRAIL, aT16, t64_1) <@ __a_ilen_read_upto8_at (
+          buf, offset, dELTA, lEN, tRAIL, 8, aT16);
+          w <- (VPINSR_2u64 w t64_1 (W8.of_int 1));
+        }
+      }
+      aT <- (cUR + aT16);
+    }
+    return (dELTA, lEN, tRAIL, aT, w);
+  }
+  proc __a_ilen_read_upto32_at (buf:W8.t A.t, offset:int, dELTA:int,
+                                lEN:int, tRAIL:int, cUR:int, aT:int) : 
+  int * int * int * int * W256.t = {
+    var w:W256.t;
+    var aT32:int;
+    var t128_0:W128.t;
+    var t128_1:W128.t;
+    if ((((aT < cUR) \/ ((cUR + 32) <= aT)) \/ ((lEN = 0) /\ (tRAIL = 0)))) {
+      w <- (set0_256);
+    } else {
+      aT32 <- (aT - cUR);
+      if (((aT32 = 0) /\ (32 <= lEN))) {
+        w <-
+        (get256_direct (WA.init8 (fun i => buf.[i])) (offset + dELTA));
+        aT32 <- (aT32 + 32);
+        dELTA <- (dELTA + 32);
+        lEN <- (lEN - 32);
+      } else {
+        if ((16 <= aT32)) {
+          w <- (set0_256);
+          (dELTA, lEN, tRAIL, aT32, t128_1) <@ __a_ilen_read_upto16_at (
+          buf, offset, dELTA, lEN, tRAIL, 16, aT32);
+          w <- (VINSERTI128 w t128_1 (W8.of_int 1));
+        } else {
+          (dELTA, lEN, tRAIL, aT32, t128_0) <@ __a_ilen_read_upto16_at (
+          buf, offset, dELTA, lEN, tRAIL, 0, aT32);
+          (dELTA, lEN, tRAIL, aT32, t128_1) <@ __a_ilen_read_upto16_at (
+          buf, offset, dELTA, lEN, tRAIL, 16, aT32);
+          w <-
+          (W256.of_int
+          (((W128.to_uint t128_0) %% (2 ^ 128)) +
+          ((2 ^ 128) * (W128.to_uint t128_1))));
+        }
+      }
+      aT <- (cUR + aT32);
+    }
+    return (dELTA, lEN, tRAIL, aT, w);
+  }
+  proc __a_ilen_read_bcast_upto8_at (buf:W8.t A.t, offset:int,
+                                     dELTA:int, lEN:int, tRAIL:int, cUR:int,
+                                     aT:int) : int * int * int * int * W256.t = {
+    var w256:W256.t;
+    var aT8:int;
+    var w:W64.t;
+    var t128:W128.t;
+    if ((((aT < cUR) \/ ((cUR + 8) <= aT)) \/ ((lEN = 0) /\ (tRAIL = 0)))) {
+      w256 <- (set0_256);
+    } else {
+      if ((8 <= lEN)) {
+        aT8 <- (aT - cUR);
+        w256 <-
+        (VPBROADCAST_4u64
+        (get64_direct (WA.init8 (fun i => buf.[i])) (offset + dELTA)));
+        w256 <@ M.__SHLQ_256 (w256, aT8);
+        dELTA <- (dELTA + (8 - aT8));
+        lEN <- (lEN - (8 - aT8));
+        aT8 <- 8;
+      } else {
+        aT8 <- (aT - cUR);
+        (dELTA, lEN, tRAIL, aT, w) <@ __a_ilen_read_upto8_at (buf, offset,
+        dELTA, lEN, tRAIL, cUR, aT);
+        t128 <- (zeroextu128 w);
+        w256 <- (VPBROADCAST_4u64 (truncateu64 t128));
+        w256 <@ M.__SHLQ_256 (w256, aT8);
+        dELTA <- (dELTA + (8 - aT8));
+        lEN <- (lEN - (8 - aT8));
+        aT8 <- 8;
+      }
+      aT <- (cUR + aT8);
+    }
+    return (dELTA, lEN, tRAIL, aT, w256);
+  }
+  proc __a_ilen_write_upto8 (buf:W8.t A.t, offset:int, dELTA:int,
+                             lEN:int, w:W64.t) : W8.t A.t * int * int = {
+    
+    if ((0 < lEN)) {
+      if ((8 <= lEN)) {
+        buf <-
+        (A.init
+        (WA.get8
+        (WA.set64_direct (WA.init8 (fun i => buf.[i]))
+        (offset + dELTA) w)));
+        dELTA <- (dELTA + 8);
+        lEN <- (lEN - 8);
+      } else {
+        if ((4 <= lEN)) {
+          buf <-
+          (A.init
+          (WA.get8
+          (WA.set32_direct (WA.init8 (fun i => buf.[i]))
+          (offset + dELTA) (truncateu32 w))));
+          w <- (w `>>` (W8.of_int 32));
+          dELTA <- (dELTA + 4);
+          lEN <- (lEN - 4);
+        } else {
+          
+        }
+        if ((2 <= lEN)) {
+          buf <-
+          (A.init
+          (WA.get8
+          (WA.set16_direct (WA.init8 (fun i => buf.[i]))
+          (offset + dELTA) (truncateu16 w))));
+          w <- (w `>>` (W8.of_int 16));
+          dELTA <- (dELTA + 2);
+          lEN <- (lEN - 2);
+        } else {
+          
+        }
+        if ((1 <= lEN)) {
+          buf <-
+          (A.init
+          (WA.get8
+          (WA.set8_direct (WA.init8 (fun i => buf.[i]))
+          (offset + dELTA) (truncateu8 w))));
+          dELTA <- (dELTA + 1);
+          lEN <- (lEN - 1);
+        } else {
+          
+        }
+      }
+    } else {
+      
+    }
+    return (buf, dELTA, lEN);
+  }
+  proc __a_ilen_write_upto16 (buf:W8.t A.t, offset:int, dELTA:int,
+                              lEN:int, w:W128.t) : W8.t A.t * int *
+                                                   int = {
+    var t64:W64.t;
+    if ((0 < lEN)) {
+      if ((16 <= lEN)) {
+        buf <-
+        (A.init
+        (WA.get8
+        (WA.set128_direct (WA.init8 (fun i => buf.[i]))
+        (offset + dELTA) w)));
+        dELTA <- (dELTA + 16);
+        lEN <- (lEN - 16);
+      } else {
+        if ((8 <= lEN)) {
+          buf <-
+          (A.init
+          (WA.get8
+          (WA.set64_direct (WA.init8 (fun i => buf.[i]))
+          (offset + dELTA) (MOVV_64 (truncateu64 w)))));
+          dELTA <- (dELTA + 8);
+          lEN <- (lEN - 8);
+          w <- (VPUNPCKH_2u64 w w);
+        } else {
+          
+        }
+        t64 <- (truncateu64 w);
+        (buf, dELTA, lEN) <@ __a_ilen_write_upto8 (buf, offset, dELTA, 
+        lEN, t64);
+      }
+    } else {
+      
+    }
+    return (buf, dELTA, lEN);
+  }
+  proc __a_ilen_write_upto32 (buf:W8.t A.t, offset:int, dELTA:int,
+                              lEN:int, w:W256.t) : W8.t A.t * int *
+                                                   int = {
+    var t128:W128.t;
+    if ((0 < lEN)) {
+      if ((32 <= lEN)) {
+        buf <-
+        (A.init
+        (WA.get8
+        (WA.set256_direct (WA.init8 (fun i => buf.[i]))
+        (offset + dELTA) w)));
+        dELTA <- (dELTA + 32);
+        lEN <- (lEN - 32);
+      } else {
+        t128 <- (truncateu128 w);
+        if ((16 <= lEN)) {
+          buf <-
+          (A.init
+          (WA.get8
+          (WA.set128_direct (WA.init8 (fun i => buf.[i]))
+          (offset + dELTA) t128)));
+          dELTA <- (dELTA + 16);
+          lEN <- (lEN - 16);
+          t128 <- (VEXTRACTI128 w (W8.of_int 1));
+        } else {
+          
+        }
+        (buf, dELTA, lEN) <@ __a_ilen_write_upto16 (buf, offset, dELTA, 
+        lEN, t128);
+      }
+    } else {
+      
+    }
+    return (buf, dELTA, lEN);
+  }
+  proc __a_rlen_read_upto8 (a:W8.t A.t, off:int, len:int) : int *
+                                                                   W64.t = {
+    var w:W64.t;
+    var zf:bool;
+    var sh:W8.t;
+    var x:W64.t;
+    var  _0:bool;
+    var  _1:bool;
+    var  _2:bool;
+    var  _3:bool;
+    var  _4:bool;
+    var  _5:bool;
+    var  _6:bool;
+    var  _7:bool;
+    var  _8:bool;
+    var  _9:bool;
+    var  _10:bool;
+    var  _11:bool;
+    if ((8 <= len)) {
+      w <- (get64_direct (WA.init8 (fun i => a.[i])) off);
+      off <- (off + 8);
+    } else {
+      ( _0,  _1,  _2,  _3, zf) <- (TEST_64 (W64.of_int len) (W64.of_int 4));
+      if ((! zf)) {
+        w <-
+        (zeroextu64 (get32_direct (WA.init8 (fun i => a.[i])) off));
+        off <- (off + 4);
+        sh <- (W8.of_int 32);
+      } else {
+        w <- (W64.of_int 0);
+        sh <- (W8.of_int 0);
+      }
+      ( _4,  _5,  _6,  _7, zf) <- (TEST_64 (W64.of_int len) (W64.of_int 2));
+      if ((! zf)) {
+        x <-
+        (zeroextu64 (get16_direct (WA.init8 (fun i => a.[i])) off));
+        x <- (x `<<` (sh `&` (W8.of_int 63)));
+        w <- (w + x);
+        off <- (off + 2);
+        sh <- (sh + (W8.of_int 16));
+      } else {
+        
+      }
+      ( _8,  _9,  _10,  _11, zf) <-
+      (TEST_64 (W64.of_int len) (W64.of_int 1));
+      if ((! zf)) {
+        x <-
+        (zeroextu64 (get8_direct (WA.init8 (fun i => a.[i])) off));
+        x <- (x `<<` (sh `&` (W8.of_int 63)));
+        w <- (w + x);
+        off <- (off + 1);
+      } else {
+        
+      }
+    }
+    return (off, w);
+  }
+  proc __a_rlen_write_upto8 (buf:W8.t A.t, off:int, data:W64.t,
+                             len:int) : W8.t A.t * int = {
+    var zf:bool;
+    var  _0:bool;
+    var  _1:bool;
+    var  _2:bool;
+    var  _3:bool;
+    var  _4:bool;
+    var  _5:bool;
+    var  _6:bool;
+    var  _7:bool;
+    var  _8:bool;
+    var  _9:bool;
+    var  _10:bool;
+    var  _11:bool;
+    if ((8 <= len)) {
+      buf <-
+      (A.init
+      (WA.get8
+      (WA.set64_direct (WA.init8 (fun i => buf.[i])) off data))
+      );
+      off <- (off + 8);
+    } else {
+      ( _0,  _1,  _2,  _3, zf) <- (TEST_64 (W64.of_int len) (W64.of_int 4));
+      if ((! zf)) {
+        buf <-
+        (A.init
+        (WA.get8
+        (WA.set32_direct (WA.init8 (fun i => buf.[i])) 
+        off (truncateu32 data))));
+        off <- (off + 4);
+        data <- (data `>>` (W8.of_int 32));
+      } else {
+        
+      }
+      ( _4,  _5,  _6,  _7, zf) <- (TEST_64 (W64.of_int len) (W64.of_int 2));
+      if ((! zf)) {
+        buf <-
+        (A.init
+        (WA.get8
+        (WA.set16_direct (WA.init8 (fun i => buf.[i])) 
+        off (truncateu16 data))));
+        off <- (off + 2);
+        data <- (data `>>` (W8.of_int 16));
+      } else {
+        
+      }
+      ( _8,  _9,  _10,  _11, zf) <-
+      (TEST_64 (W64.of_int len) (W64.of_int 1));
+      if ((! zf)) {
+        buf <-
+        (A.init
+        (WA.get8
+        (WA.set8_direct (WA.init8 (fun i => buf.[i])) off
+        (truncateu8 data))));
+        off <- (off + 1);
+      } else {
+        
+      }
+    }
+    return (buf, off);
+  }
+}.
+
+lemma a_ilen_read_upto8_at_ll: islossless MM.__a_ilen_read_upto8_at
+by islossless.
+
+lemma a_ilen_read_upto16_at_ll: islossless MM.__a_ilen_read_upto16_at
+by islossless.
+
+lemma a_ilen_read_upto32_at_ll: islossless MM.__a_ilen_read_upto32_at
+by islossless.
+
+lemma a_ilen_read_bcast_upto8_at_ll: islossless MM.__a_ilen_read_bcast_upto8_at
+by islossless.
+
+lemma a_ilen_write_upto8_ll: islossless MM.__a_ilen_write_upto8
+by islossless.
+
+lemma a_ilen_write_upto16_ll: islossless MM.__a_ilen_write_upto8
+by islossless.
+
+lemma a_ilen_write_upto32_ll: islossless MM.__a_ilen_write_upto32
+by islossless.
+
+lemma a_rlen_read_upto8_ll: islossless MM.__a_rlen_read_upto8
+by islossless.
+
+lemma a_rlen_write_upto8_ll: islossless MM.__a_rlen_write_upto8
+by islossless.
+
+
+end ReadWriteArray.
