proof/amd64/extracted/Keccak1600_fixedsizes_avx2_checkXtr.ec
@@ -1,0 +1,38 @@
+require import AllCore IntDiv List.
+
+from Jasmin require import JModel.
+
+(** This script performs a sanity check to verify if the modules
+ used for correctness proofs are in sync. with the Jasmin source code *)
+
+from JazzEC require import Keccak1600_Jazz_ASIZE.
+from JazzEC require import Array999 WArray999.
+
+require import Keccak1600_fixedsizes_avx2.
+
+clone import KeccakArrayAvx2 as A999avx2
+ with op _ASIZE <- 999,
+      theory A <- Array999,
+      theory WA <- WArray999
+      proof _ASIZE_ge0 by done.
+
+equiv a999_addstate_avx2_eq:
+ M.__addstate_avx2 ~ MM.__addstate_avx2
+ : ={arg} ==> ={res}
+by sim.
+
+equiv a999_absorb_avx2_eq:
+ M.__absorb_avx2 ~ MM.__absorb_avx2
+ : ={arg} ==> ={res}
+by sim.
+
+equiv a999_dumpstate_avx2_eq:
+ M.__dumpstate_avx2 ~ MM.__dumpstate_avx2
+ : ={arg} ==> ={res}
+by sim.
+
+equiv a999_squeeze_avx2_eq:
+ M.__squeeze_avx2 ~ MM.__squeeze_avx2
+ : ={arg} ==> ={res}
+by sim.
+
