proof/amd64/extracted/Keccak1600_fixedsizes_avx2x4_checkXtr.ec
@@ -1,0 +1,48 @@
+require import AllCore IntDiv List.
+
+from Jasmin require import JModel.
+
+(** This script performs a sanity check to verify if the modules
+ used for correctness proofs are in sync. with the Jasmin source code *)
+
+from JazzEC require import Keccak1600_Jazz_ASIZE.
+from JazzEC require import Array999 WArray999.
+
+require import Keccak1600_fixedsizes_avx2x4.
+
+clone import KeccakArrayAvx2x4 as A999avx2x4
+ with op _ASIZE <- 999,
+      theory A <- Array999,
+      theory WA <- WArray999
+      proof _ASIZE_ge0 by done.
+
+equiv a999_addstate_bcast_avx2x4_eq:
+ M.__addstate_bcast_avx2x4 ~ MM.__addstate_bcast_avx2x4
+ : ={arg} ==> ={res}
+by sim.
+
+equiv a999_addstate_avx2x4_eq:
+ M.__addstate_avx2x4 ~ MM.__addstate_avx2x4
+ : ={arg} ==> ={res}
+by sim.
+
+equiv a999_absorb_bcast_avx2x4_eq:
+ M.__absorb_bcast_avx2x4 ~ MM.__absorb_bcast_avx2x4
+ : ={arg} ==> ={res}
+by sim.
+
+equiv a999_absorb_avx2x4_eq:
+ M.__absorb_avx2x4 ~ MM.__absorb_avx2x4
+ : ={arg} ==> ={res}
+by sim.
+
+equiv a999_dumpstate_avx2_eq:
+ M.__dumpstate_avx2x4 ~ MM.__dumpstate_avx2x4
+ : ={arg} ==> ={res}
+by sim.
+
+equiv a999_squeeze_avx2x4_eq:
+ M.__squeeze_avx2x4 ~ MM.__squeeze_avx2x4
+ : ={arg} ==> ={res}
+by sim.
+
