proof/amd64/extracted/Keccak1600_subreadwrite_checkXtr.ec
@@ -1,0 +1,63 @@
+require import AllCore IntDiv List.
+
+from Jasmin require import JModel.
+
+(** This script performs a sanity check to verify if the modules
+ used for correctness proofs are in sync. with the Jasmin source code *)
+
+from JazzEC require import Keccak1600_Jazz_ASIZE.
+from JazzEC require import Array999 WArray999.
+
+require import Keccak1600_subreadwrite.
+
+clone import ReadWriteArray as A999ref
+ with op _ASIZE <- 999,
+      theory A <- Array999,
+      theory WA <- WArray999
+      proof _ASIZE_ge0 by done.
+
+equiv a999_a_ilen_read_upto8_at_eq:
+ M.__a_ilen_read_upto8_at ~ MM.__a_ilen_read_upto8_at
+ : ={arg} ==> ={res}
+by sim.
+
+equiv a999_a_ilen_read_upto16_at_eq:
+ M.__a_ilen_read_upto16_at ~ MM.__a_ilen_read_upto16_at
+ : ={arg} ==> ={res}
+by sim.
+
+equiv a999_a_ilen_read_upto32_at_eq:
+ M.__a_ilen_read_upto32_at ~ MM.__a_ilen_read_upto32_at
+ : ={arg} ==> ={res}
+by sim.
+
+equiv a999_a_ilen_read_bcast_upto8_at_eq:
+ M.__a_ilen_read_bcast_upto8_at ~ MM.__a_ilen_read_bcast_upto8_at
+ : ={arg} ==> ={res}
+by sim.
+
+equiv a999_a_ilen_write_upto8_eq:
+ M.__a_ilen_write_upto8 ~ MM.__a_ilen_write_upto8
+ : ={arg} ==> ={res}
+by sim.
+
+equiv a999_a_ilen_write_upto16_eq:
+ M.__a_ilen_write_upto16 ~ MM.__a_ilen_write_upto16
+ : ={arg} ==> ={res}
+by sim.
+
+equiv a999_a_ilen_write_upto32_eq:
+ M.__a_ilen_write_upto32 ~ MM.__a_ilen_write_upto32
+ : ={arg} ==> ={res}
+by sim.
+
+equiv a999_a_rlen_read_upto8_eq:
+ M.__a_rlen_read_upto8 ~ MM.__a_rlen_read_upto8
+ : ={arg} ==> ={res}
+by sim.
+
+equiv a999_a_rlen_write_upto8_eq:
+ M.__a_rlen_write_upto8 ~ MM.__a_rlen_write_upto8
+ : ={arg} ==> ={res}
+by sim.
+
