proof/amd64/ref/Keccak1600_fixedsizes_ref.ec
@@ -1,0 +1,534 @@
+(******************************************************************************
+   Keccak1600_imem_ref.ec:
+
+   Correctness proof for the Keccak (fixed-sized) memory absorb/squeeze
+  REF implementation
+
+
+
+******************************************************************************)
+
+require import List Real Distr Int IntDiv CoreMap.
+
+from Jasmin require import JModel.
+
+from CryptoSpecs require export Keccakf1600_Spec.
+
+from JazzEC require import Keccak1600_Jazz.
+
+from JazzEC require import WArray200.
+from JazzEC require import Array25.
+
+from CryptoSpecs require import JWordList.
+from CryptoSpecs require import FIPS202_Keccakf1600.
+from CryptoSpecs require import FIPS202_SHA3_Spec Keccakf1600_Spec.
+
+
+require import Keccak1600_ref Keccakf1600_ref.
+require import Keccak1600_subreadwrite.
+
+
+(*
+   ONE-SHOT (FIXED-SIZE) MEMORY ABSORB
+   ===================================
+*)
+
+lemma addstate_m_ref_ll: islossless M.__addstate_m_ref.
+proof.
+islossless.
+while true (aT %/ 8 + _LEN %/ 8 - at).
+ by move=> z; auto; smt().
+by auto; smt().
+qed.
+
+hoare addstate_m_ref_h _mem _st _at _buf _len _tb:
+ M.__addstate_m_ref
+ : Glob.mem=_mem /\ st=_st /\ aT=_at /\ buf=_buf /\ _LEN=_len /\ _TRAILB=_tb
+ /\ 0 <= _at <= 200
+ /\ 0 <= _len
+ /\ _at+_len <= 200 - b2i (_tb<>0)
+ /\ _buf + _len < W64.modulus
+ ==> let l = memread _mem _buf _len ++ if _tb<>0 then [W8.of_int _tb] else []
+  in Glob.mem=_mem
+  /\ res.`1 = addstate_at _st _at l
+  /\ res.`2 = _at + size l
+  /\ res.`3 = _buf + _len.
+proof.
+admitted.
+
+phoare addstate_m_ref_ph _mem _st _at _buf _len _tb:
+ [ M.__addstate_m_ref
+ : Glob.mem=_mem /\ st=_st /\ aT=_at /\ buf=_buf /\ _LEN=_len /\ _TRAILB=_tb
+ /\ 0 <= _at <= 200
+ /\ 0 <= _len
+ /\ _at+_len <= 200 - b2i (_tb<>0)
+ /\ _buf + _len < W64.modulus
+ ==> let l = memread _mem _buf _len ++ if _tb<>0 then [W8.of_int _tb] else []
+  in Glob.mem=_mem
+  /\ res.`1 = addstate_at _st _at l
+  /\ res.`2 = _at + size l
+  /\ res.`3 = _buf + _len
+ ] = 1%r.
+proof.
+by conseq addstate_m_ref_ll (addstate_m_ref_h _mem _st _at _buf _len _tb).
+qed.
+
+lemma absorb_m_ref_ll: islossless M.__absorb_m_ref.
+proof.
+proc; simplify.
+seq 2: true => //.
+ call addstate_m_ref_ll.
+ if => //.
+ wp; while true (iTERS-i).
+  move=> z; auto.
+  call keccakf1600_ref_ll.
+  call addstate_m_ref_ll.
+  by auto => /#.
+ wp; call keccakf1600_ref_ll.
+ wp; call addstate_m_ref_ll.
+ by auto => /#.
+if => //.
+by call addratebit_ref_ll.
+qed.
+
+hoare absorb_m_ref_h _l _mem _buf _len _r8 _tb:
+ M.__absorb_m_ref
+ : Glob.mem=_mem /\ aT=size _l %% _r8 /\ buf=_buf /\ _LEN=_len /\ _RATE8=_r8 /\ _TRAILB=_tb
+ /\ pabsorb_spec_ref _r8 _l st
+ /\ 0 <= _len
+ /\ _buf + _len < W64.modulus
+ ==> Glob.mem = _mem
+  /\ if _tb <> 0
+     then res.`1 = ABSORB1600 (W8.of_int _tb) _r8 (_l ++ memread _mem _buf _len)
+       /\ res.`3 = _buf + _len
+     else pabsorb_spec_ref _r8 (_l ++ memread _mem _buf _len) res.`1
+       /\ res.`2 = (size _l + _len) %% _r8
+       /\ res.`3 = _buf + _len.
+proof.
+proc.
+admitted.
+
+phoare absorb_m_ref_ph _l _mem _buf _len _r8 _tb:
+ [ M.__absorb_m_ref
+ : Glob.mem=_mem /\ aT=size _l %% _r8 /\ buf=_buf /\ _LEN=_len /\ _RATE8=_r8 /\ _TRAILB=_tb
+ /\ pabsorb_spec_ref _r8 _l st
+ /\ 0 <= _len
+ /\ _buf + _len < W64.modulus
+ ==> Glob.mem = _mem
+  /\ if _tb <> 0
+     then res.`1 = ABSORB1600 (W8.of_int _tb) _r8 (_l ++ memread _mem _buf _len)
+       /\ res.`3 = _buf + (max 0 _len)
+     else pabsorb_spec_ref _r8 (_l ++ memread _mem _buf _len) res.`1
+       /\ res.`2 = (size _l + _len) %% _r8
+       /\ res.`3 = _buf + _len
+ ] = 1%r.
+proof.
+by conseq absorb_m_ref_ll (absorb_m_ref_h _l _mem _buf _len _r8 _tb) => /> /#.
+qed.
+
+(*
+   ONE-SHOT (FIXED-SIZE) MEMORY SQUEEZE
+   ====================================
+*)
+
+lemma dumpstate_m_ref_ll: islossless M.__dumpstate_m_ref.
+proof.
+proc => /=.
+seq 2: true => //.
+ while true (_LEN %/ 8 - i).
+  by move=> z; auto => /#. 
+ by auto => /#.
+by islossless.
+qed.
+
+hoare dumpstate_m_ref_h _mem _buf _len _st:
+ M.__dumpstate_m_ref
+ : Glob.mem=_mem /\ buf=_buf /\ _LEN=_len /\ st=_st
+ /\ 0 <= _len <= 200
+ /\ _buf + _len < W64.modulus
+ ==> Glob.mem = stores _mem _buf (sub (stbytes _st) 0 _len)
+  /\ res = _buf + _len.
+proof.
+proc => /=.
+admitted.
+
+phoare dumpstate_m_ref_ph _mem _buf _len _st:
+ [ M.__dumpstate_m_ref
+ : Glob.mem=_mem /\ buf=_buf /\ _LEN=_len /\ st=_st
+ /\ 0 <= _len <= 200
+ /\ _buf + _len < W64.modulus
+ ==> Glob.mem = stores _mem _buf (sub (stbytes _st) 0 _len)
+  /\ res = _buf + _len
+ ] = 1%r.
+proof.
+by conseq dumpstate_m_ref_ll (dumpstate_m_ref_h _mem _buf _len _st).
+qed.
+
+lemma squeeze_m_ref_ll: islossless M.__squeeze_m_ref.
+proof.
+proc; simplify.
+seq 2: true => //.
+ while true (_LEN %/ _RATE8 - i).
+  move => z; auto => />.
+  call dumpstate_m_ref_ll.
+  call keccakf1600_ref_ll.
+  by auto => /#.
+ by auto => /#.
+if => //.
+call dumpstate_m_ref_ll.
+call keccakf1600_ref_ll.
+by auto => /#.
+qed.
+
+hoare squeeze_m_ref_h _mem _buf _len _st _r8:
+ M.__squeeze_m_ref
+ : Glob.mem=_mem /\ buf=_buf /\ _LEN=_len /\ st=_st /\ _RATE8=_r8
+ /\ 0 <= _len
+ /\ 0 < _r8 <= 200
+ /\ _buf + _len < W64.modulus
+ ==> Glob.mem = stores _mem _buf (SQUEEZE1600 _r8 _len _st)
+     /\ res.`1 = st_i _st ((_len-1) %/ _r8 + 1)
+     /\ res.`2 = _buf + _len.
+proof.
+proc.
+admitted.
+
+phoare squeeze_m_ref_ph _mem _buf _len _st _r8:
+ [ M.__squeeze_m_ref
+ : Glob.mem=_mem /\ buf=_buf /\ _LEN=_len /\ st=_st /\ _RATE8=_r8
+ /\ 0 <= _len
+ /\ 0 < _r8 <= 200
+ /\ _buf + _len < W64.modulus
+ ==> Glob.mem = stores _mem _buf (SQUEEZE1600 _r8 _len _st)
+     /\ res.`1 = st_i _st ((_len-1) %/ _r8 + 1)
+     /\ res.`2 = _buf + _len
+ ] = 1%r.
+proof.
+by conseq squeeze_m_ref_ll (squeeze_m_ref_h _mem _buf _len _st _r8).
+qed.
+
+
+
+abstract theory KeccakArrayRef.
+
+op _ASIZE: int.
+
+axiom _ASIZE_ge0: 0 <= _ASIZE.
+axiom _ASIZE_u64: _ASIZE < W64.modulus.
+
+(*
+module type MParam = {
+  proc keccakf1600_ref (a:W64.t Array25.t) : W64.t Array25.t
+  proc state_init_ref (st:W64.t Array25.t) : W64.t Array25.t
+  proc addratebit_ref (st:W64.t Array25.t, _RATE8:int) : W64.t Array25.t
+}.
+*)
+
+clone import PolyArray as A
+ with op size <- _ASIZE
+      proof ge0_size by exact _ASIZE_ge0.
+
+clone import WArray as WA
+ with op size <- _ASIZE.
+
+clone import ReadWriteArray as RW
+ with op _ASIZE <- _ASIZE,
+      theory A <- A,
+      theory WA <- WA
+      proof _ASIZE_ge0 by exact _ASIZE_ge0
+      proof _ASIZE_u64 by exact _ASIZE_u64.
+
+
+module MM = {
+  proc __addstate_ref (st:W64.t Array25.t, aT:int, buf:W8.t A.t,
+                       offset:int, _LEN:int, _TRAILB:int) : W64.t Array25.t *
+                                                            int * int = {
+    var dELTA:int;
+    var aT8:int;
+    var w:W64.t;
+    var at:int;
+    dELTA <- 0;
+    aT8 <- aT;
+    aT <- (8 * (aT %/ 8));
+    if ((aT8 <> 0)) {
+      (dELTA, _LEN, _TRAILB, aT8, w) <@ RW.MM.__a_ilen_read_upto8_at (buf, 
+      offset, dELTA, _LEN, _TRAILB, aT, aT8);
+      st.[(aT %/ 8)] <- (st.[(aT %/ 8)] `^` w);
+      aT <- aT8;
+    } else {
+      
+    }
+    offset <- (offset + dELTA);
+    at <- (aT %/ 8);
+    while ((at < ((aT %/ 8) + (_LEN %/ 8)))) {
+      w <- (get64_direct (WA.init8 (fun i => buf.[i])) offset);
+      offset <- (offset + 8);
+      st.[at] <- (st.[at] `^` w);
+      at <- (at + 1);
+    }
+    aT <- (aT + (8 * (_LEN %/ 8)));
+    _LEN <- (_LEN %% 8);
+    if (((0 < _LEN) \/ ((_TRAILB %% 256) <> 0))) {
+      (dELTA, _LEN, _TRAILB, aT, w) <@ RW.MM.__a_ilen_read_upto8_at (buf, offset,
+      0, _LEN, _TRAILB, aT, aT);
+      st.[at] <- (st.[at] `^` w);
+      offset <- (offset + dELTA);
+    } else {
+      
+    }
+    return (st, aT, offset);
+  }
+  proc __absorb_ref (st:W64.t Array25.t, aT:int, buf:W8.t A.t,
+                     _TRAILB:int, _RATE8:int) : W64.t Array25.t * int = {
+    var _LEN:int;
+    var iTERS:int;
+    var offset:int;
+    var i:int;
+    var  _0:int;
+    var  _1:int;
+    var  _2:int;
+    offset <- 0;
+    _LEN <- _ASIZE;
+    if ((_RATE8 <= (aT + _LEN))) {
+      (st,  _0, offset) <@ __addstate_ref (st, aT, buf, offset,
+      (_RATE8 - aT), 0);
+      _LEN <- (_LEN - (_RATE8 - aT));
+      aT <- 0;
+      (* Erased call to spill *)
+      st <@ M._keccakf1600_ref (st);
+      (* Erased call to unspill *)
+      iTERS <- (_LEN %/ _RATE8);
+      i <- 0;
+      while ((i < iTERS)) {
+        (st,  _1, offset) <@ __addstate_ref (st, 0, buf, offset, _RATE8, 0);
+        (* Erased call to spill *)
+        st <@ M._keccakf1600_ref (st);
+        (* Erased call to unspill *)
+        i <- (i + 1);
+      }
+      _LEN <- (_LEN %% _RATE8);
+    } else {
+      
+    }
+    (st, aT,  _2) <@ __addstate_ref (st, aT, buf, offset, _LEN, _TRAILB);
+    if ((_TRAILB <> 0)) {
+      st <@ M.__addratebit_ref (st, _RATE8);
+    } else {
+      
+    }
+    return (st, aT);
+  }
+  proc __dumpstate_ref (buf:W8.t A.t, offset:int, _LEN:int,
+                        st:W64.t Array25.t) : W8.t A.t * int = {
+    var t:W64.t;
+    var dELTA:int;
+    var i:int;
+    var  _0:int;
+    i <- 0;
+    while ((i < (_LEN %/ 8))) {
+      t <- st.[i];
+      buf <-
+      (A.init
+      (WA.get8
+      (WA.set64_direct (WA.init8 (fun i_0 => buf.[i_0])) 
+      offset t)));
+      offset <- (offset + 8);
+      i <- (i + 1);
+    }
+    if ((0 < (_LEN %% 8))) {
+      t <- st.[i];
+      (buf, dELTA,  _0) <@ RW.MM.__a_ilen_write_upto8 (buf, offset, 0, (_LEN %% 8),
+      t);
+      offset <- (offset + dELTA);
+    } else {
+      
+    }
+    return (buf, offset);
+  }
+  proc __squeeze_ref (st:W64.t Array25.t, buf:W8.t A.t, _RATE8:int) : 
+  W64.t Array25.t * W8.t A.t = {
+    var offset:int;
+    var i:int;
+    offset <- 0;
+    i <- 0;
+    while ((i < (_ASIZE %/ _RATE8))) {
+      (* Erased call to spill *)
+      st <@ M._keccakf1600_ref (st);
+      (* Erased call to unspill *)
+      (buf, offset) <@ __dumpstate_ref (buf, offset, _RATE8, st);
+      (* Erased call to unspill *)
+      i <- (i + 1);
+    }
+    if ((0 < (_ASIZE %% _RATE8))) {
+      (* Erased call to spill *)
+      st <@ M._keccakf1600_ref (st);
+      (* Erased call to unspill *)
+      (buf, offset) <@ __dumpstate_ref (buf, offset, (_ASIZE %% _RATE8), st);
+    } else {
+      
+    }
+    return (st, buf);
+  }
+}.
+
+lemma addstate_ref_ll: islossless MM.__addstate_ref.
+proof.
+islossless.
+while true (aT %/ 8 + _LEN %/ 8 - at).
+ by move=> z; auto; smt().
+by auto; smt().
+qed.
+
+hoare addstate_ref_h _st _at _buf _off _len _tb:
+ MM.__addstate_ref
+ : st=_st /\ aT=_at /\ buf=_buf /\ offset=_off /\ _LEN=_len /\ _TRAILB=_tb
+ /\ 0 <= _at <= 200
+ /\ 0 <= _len
+ /\ _at + _len <= 200 - b2i (_tb<>0)
+ /\ offset + _len <= _ASIZE
+ ==> let l = sub _buf _off _len ++ if _tb <> 0 then [W8.of_int _tb] else []
+     in res.`1 = addstate_at _st _at l
+     /\ res.`2 = _at + size l
+     /\ res.`3 = _off + _len.
+proof.
+proc => /=.
+admitted.
+
+phoare addstate_ref_ph _st _at _buf _off _len _tb:
+ [ MM.__addstate_ref
+   : st=_st /\ aT=_at /\ buf=_buf /\ offset=_off /\ _LEN=_len /\ _TRAILB=_tb
+   /\ 0 <= _at <= 200
+   /\ 0 <= _len
+   /\ _at + _len <= 200 - b2i (_tb<>0)
+   /\ offset + _len <= _ASIZE
+   ==> let l = sub _buf _off _len ++ if _tb <> 0 then [W8.of_int _tb] else []
+       in res.`1 = addstate_at _st _at l
+       /\ res.`2 = _at + size l
+       /\ res.`3 = _off + _len] = 1%r.
+proof.
+by conseq addstate_ref_ll (addstate_ref_h _st _at _buf _off _len _tb).
+qed.
+
+lemma absorb_ref_ll: islossless MM.__absorb_ref.
+proof.
+proc; simplify.
+seq 4: true => //.
+ call addstate_ref_ll.
+ sp 2; if => //.
+ wp; while true (iTERS-i).
+  move=> z; auto.
+  call keccakf1600_ref_ll.
+  call addstate_ref_ll.
+  by auto => /#.
+ wp; call keccakf1600_ref_ll.
+ wp; call addstate_ref_ll.
+ by auto => /#.
+if => //.
+by call addratebit_ref_ll.
+qed.
+
+hoare absorb_ref_h _l _buf _r8 _tb:
+ MM.__absorb_ref
+ : aT=size _l %% _r8 /\ buf=_buf /\ _RATE8=_r8 /\ _TRAILB=_tb
+ /\ pabsorb_spec_ref _r8 _l st
+ ==> if _tb <> 0
+     then res.`1 = ABSORB1600 (W8.of_int _tb) _r8 (_l ++ to_list _buf)
+     else pabsorb_spec_ref _r8 (_l ++ to_list _buf) res.`1
+       /\ res.`2 = (size _l + _ASIZE) %% _r8.
+proof.
+proc.
+admitted.
+
+phoare absorb_ref_ph _l _buf _r8 _tb:
+ [ MM.__absorb_ref
+ : aT=size _l %% _r8 /\ buf=_buf /\ _RATE8=_r8 /\ _TRAILB=_tb
+ /\ pabsorb_spec_ref _r8 _l st
+ ==> if _tb <> 0
+     then res.`1 = ABSORB1600 (W8.of_int _tb) _r8 (_l ++ to_list _buf)
+     else pabsorb_spec_ref _r8 (_l ++ to_list _buf) res.`1
+       /\ res.`2 = (size _l + _ASIZE) %% _r8
+ ] = 1%r.
+proof.
+by conseq absorb_ref_ll (absorb_ref_h _l _buf _r8 _tb); smt(ge0_size).
+qed.
+
+(*
+   ONE-SHOT (FIXED-SIZE) MEMORY SQUEEZE
+   ====================================
+*)
+
+lemma dumpstate_ref_ll: islossless MM.__dumpstate_ref.
+proof.
+proc => /=.
+seq 2: true => //.
+ while true (_LEN %/ 8 - i).
+  by move=> z; auto => /#. 
+ by auto => /#.
+by islossless.
+qed.
+
+hoare dumpstate_ref_h _buf _off _len _st:
+ MM.__dumpstate_ref
+ : buf=_buf /\ offset=_off /\ _LEN=_len /\ st=_st
+ /\ 0 <= _len <= 200
+ /\ _off + _len <= _ASIZE
+ ==> res.`1 = A.fill (fun i=>(stbytes _st).[i-_off]) _off _len _buf
+  /\ res.`2 = _off + _len.
+proof.
+proc.
+admitted.
+
+phoare dumpstate_ref_ph _buf _off _len _st:
+ [ MM.__dumpstate_ref
+ : buf=_buf /\ offset=_off /\ _LEN=_len /\ st=_st
+ /\ 0 <= _len <= 200
+ /\ _off + _len <= _ASIZE
+ ==> res.`1 = A.fill (fun i=>(stbytes _st).[i-_off]) _off _len _buf
+  /\ res.`2 = _off + _len
+ ] = 1%r.
+proof.
+have ?:= dumpstate_ref_ll.
+have ?:= (dumpstate_ref_h _buf _off _len _st).
+admit (* ????? anomaly: EcLib.EcCoreGoal.InvalidGoalShape ????
+by conseq dumpstate_ref_ll (dumpstate_ref_h _buf _off _len _st).
+*).
+qed.
+
+lemma squeeze_ref_ll: islossless MM.__squeeze_ref.
+proof.
+proc; simplify.
+seq 3: true => //.
+ while true (_ASIZE %/ _RATE8 - i).
+  move => z; auto => />.
+  call dumpstate_ref_ll.
+  call keccakf1600_ref_ll.
+  by auto => /#.
+ by auto => /#.
+if => //.
+call dumpstate_ref_ll.
+call keccakf1600_ref_ll.
+by auto => /#.
+qed.
+
+hoare squeeze_ref_h _buf _st _r8:
+ MM.__squeeze_ref
+ : buf=_buf /\ st=_st /\ _RATE8=_r8
+ /\ 0 < _r8 <= 200
+ ==> res.`1 = st_i _st ((_ASIZE-1) %/ _r8 + 1)
+     /\ to_list res.`2 = (SQUEEZE1600 _r8 _ASIZE _st).
+proof.
+proc.
+admitted.
+
+phoare squeeze_ref_ph _buf _st _r8:
+ [ MM.__squeeze_ref
+ : buf=_buf /\ st=_st /\ _RATE8=_r8
+ /\ 0 < _r8 <= 200
+ ==> res.`1 = st_i _st ((_ASIZE-1) %/ _r8 + 1)
+     /\ to_list res.`2 = (SQUEEZE1600 _r8 _ASIZE _st)
+ ] = 1%r.
+proof.
+by conseq squeeze_ref_ll (squeeze_ref_h _buf _st _r8).
+qed.
+
+end KeccakArrayRef.
