Makefile
@@ -1,0 +1,21 @@
+# -*- Makefile -*-
+
+# --------------------------------------------------------------------
+ECCONF := config/tests.config 
+CHECKS ?= keccak
+
+# --------------------------------------------------------------------
+.PHONY: default check checkec jasmin assembly clean_eco
+
+default: check
+
+check: jasmin checkec
+
+jasmin:
+	make -C proof/amd64/extracted
+
+checkec:
+	easycrypt runtest $(ECCONF) $(CHECKS)
+
+clean_eco:
+	find proof -name '*.eco' -exec rm '{}' ';'
